\SetValue{Module}{1}\SetValue{SectionAB}{A}\SetValue{MainChapter}{}\SetValue{SubChapter}{}\SetValue{Contents}{%%
    
Determine whether the geometric series is convergent or divergent. If it is convergent, find its sum.

$$\sum_{n=1}^{\infty} \dfrac{(-3)^{n-1}}{4^n}$$


}\SetValue{Concept}{%



}\SetValue{AltText}{%



}\SetValue{Solution}{%

Step 1: Rewrite the general term

We aim to express this in geometric series form: $a \cdot r^{n-1}$
Start by separating powers:

$$
\dfrac{(-3)^{n-1}}{4^n}=\dfrac{1}{4} \cdot\left(\dfrac{-3}{4}\right)^{n-1}
$$


So the series becomes:

$$
\sum_{n=1}^{\infty} \dfrac{1}{4}\left(\dfrac{-3}{4}\right)^{n-1}
$$


This is a geometric series with:

- First term $a=\dfrac{1}{4}$

- Common ratio $r=\dfrac{-3}{4}$

Step 2: Convergence test

A geometric series $\sum a r^{n-1}$ converges if $|r|<1$.
Here:

$$
|r|=\left|\dfrac{-3}{4}\right|=\dfrac{3}{4}<1
$$

The series converges.

Step 3: Use the geometric series sum formula

$$
S=\dfrac{a}{1-r}=\dfrac{\dfrac{1}{4}}{1-\left(-\dfrac{3}{4}\right)}=\dfrac{\dfrac{1}{4}}{1+\dfrac{3}{4}}=\dfrac{\dfrac{1}{4}}{\dfrac{7}{4}}=\dfrac{1}{7}
$$


Final Answer:

- The series is convergent.

- The sum is $\dfrac{1}{7}$.

}\SetValue{Rubric}{%Markdown



}\SetValue{Hint}{%
Solution Goes Here
}\SetValue{Answer}{%

}
\ProcessDATA



