\SetValue{Module}{1}\SetValue{SectionAB}{A}\SetValue{MainChapter}{}\SetValue{SubChapter}{}\SetValue{Contents}{%%
    
Determine whether the geometric series is convergent or divergent. If it is convergent, find its sum.

$$\sum_{n=1}^{\infty} \dfrac{e^n}{3^{n-1}}$$

}\SetValue{Concept}{%



}\SetValue{AltText}{%



}\SetValue{Solution}{%

Step 1: Rewrite the general term

We want to express the term in geometric form: $a \cdot r^{n-1}$

$$
\dfrac{e^n}{3^{n-1}}=e \cdot\left(\dfrac{e}{3}\right)^{n-1}
$$


So the series becomes:

$$
\sum_{n=1}^{\infty} e\left(\dfrac{e}{3}\right)^{n-1}
$$


This is a geometric series with:

- First term: $a=e$

- Common ratio: $r=\dfrac{e}{3}$

Step 2: Convergence Test

A geometric series $\sum a r^{n-1}$ converges if and only if $|r|<1$

Here:

- $e \approx 2.718$

- So $\dfrac{e}{3} \approx 0.906<1$

Therefore, the series converges

Step 3: Use the geometric series sum formula

$$
S=\dfrac{a}{1-r}=\dfrac{e}{1-\dfrac{e}{3}}=\dfrac{e}{\dfrac{3-e}{3}}=\dfrac{3 e}{3-e}
$$

Final Answer:

- The series is convergent

- The sum is:

$$
\dfrac{3 e}{3-e}
$$

}\SetValue{Rubric}{%Markdown



}\SetValue{Hint}{%
Solution Goes Here
}\SetValue{Answer}{%

}
\ProcessDATA



