\SetValue{Module}{1}\SetValue{SectionAB}{A}\SetValue{MainChapter}{}\SetValue{SubChapter}{}\SetValue{Contents}{%%
    
Determine whether the series is convergent or divergent. If it is convergent, find its sum.

$$\sum_{n=1}^{\infty}\left[(0.8)^{n-1}-(0.3)^n\right]$$


}\SetValue{Concept}{%



}\SetValue{AltText}{%



}\SetValue{Solution}{%

Step 1: Split the Series

This is the sum of two series:

$$
\sum_{n=1}^{\infty}(0.8)^{n-1}-\sum_{n=1}^{\infty}(0.3)^n
$$


Step 2: Evaluate Each Series

1. First series: $\sum_{n=1}^{\infty}(0.8)^{n-1}$

Let's shift the index so it becomes a standard geometric series:

Let $m=n-1$, so when $n=1, m=0$ :

$$
\sum_{n=1}^{\infty}(0.8)^{n-1}=\sum_{m=0}^{\infty}(0.8)^m
$$


This is a geometric series with:

- First term $a=1$

- Common ratio $r=0.8$

$$
\sum=\dfrac{1}{1-0.8}=\dfrac{1}{0.2}=5
$$

2. Second series: $\sum_{n=1}^{\infty}(0.3)^n$

This is also a geometric series:

- First term $a=0.3$

- Common ratio $r=0.3$

$$
\sum=\dfrac{0.3}{1-0.3}=\dfrac{0.3}{0.7}=\dfrac{3}{7}
$$


Step 3: Subtract the Two Sums

$$
\sum_{n=1}^{\infty}\left[(0.8)^{n-1}-(0.3)^n\right]=5-\dfrac{3}{7}=\dfrac{35-3}{7}=\dfrac{32}{7}
$$


Final Answer:

$$
\dfrac{32}{7}
$$


}\SetValue{Rubric}{%Markdown



}\SetValue{Hint}{%
Solution Goes Here
}\SetValue{Answer}{%

}
\ProcessDATA



