\SetValue{Module}{1}\SetValue{SectionAB}{A}\SetValue{MainChapter}{}\SetValue{SubChapter}{}\SetValue{Contents}{%%
    
Determine whether the series is convergent or divergent. If it is convergent, find its sum.

$$\sum_{n=1}^{\infty}\left(\dfrac{1}{e^n}+\dfrac{1}{n(n+1)}\right)$$

}\SetValue{Concept}{%



}\SetValue{AltText}{%



}\SetValue{Solution}{%

Step 1: Break it into two series

$$
\sum_{n=1}^{\infty}\left(\dfrac{1}{e^n}+\dfrac{1}{n(n+1)}\right)=\sum_{n=1}^{\infty} \dfrac{1}{e^n}+\sum_{n=1}^{\infty} \dfrac{1}{n(n+1)}
$$


We will analyze both parts.

Step 2: Convergence of $\sum \dfrac{1}{e^n}$

This is a geometric series:

- $a=\dfrac{1}{e}, r=\dfrac{1}{e}<1$

- It converges, and the sum is:

$$
\sum_{n=1}^{\infty} \dfrac{1}{e^n}=\dfrac{\dfrac{1}{e}}{1-\dfrac{1}{e}}=\dfrac{1}{e-1}
$$


Step 3: Convergence and Sum of $\sum \dfrac{1}{n(n+1)}$

This is a telescoping series:

$$
\dfrac{1}{n(n+1)}=\dfrac{1}{n}-\dfrac{1}{n+1}
$$

So:

$$
\sum_{n=1}^{\infty}\left(\dfrac{1}{n}-\dfrac{1}{n+1}\right)=\left(1-\dfrac{1}{2}\right)+\left(\dfrac{1}{2}-\dfrac{1}{3}\right)+\left(\dfrac{1}{3}-\dfrac{1}{4}\right)+\cdots
$$


This telescopes nicely:

$$
\sum_{n=1}^{\infty} \dfrac{1}{n(n+1)}=1
$$


Step 4: Add the Two Results

$$
\sum_{n=1}^{\infty}\left(\dfrac{1}{e^n}+\dfrac{1}{n(n+1)}\right)=\dfrac{1}{e-1}+1
$$


Final Answer:

- The series converges.

- The sum is: $1+\dfrac{1}{e-1}$

}\SetValue{Rubric}{%Markdown



}\SetValue{Hint}{%
Solution Goes Here
}\SetValue{Answer}{%

}
\ProcessDATA



