\SetValue{Module}{1}\SetValue{SectionAB}{A}\SetValue{MainChapter}{}\SetValue{SubChapter}{}\SetValue{Contents}{%%
    
Determine whether the series is convergent or divergent by expressing $s_n$ as a telescoping sum. If it is convergent, find its sum.

$$\sum_{n=1}^{\infty} \ln \dfrac{n}{n+1}$$

}\SetValue{Concept}{%



}\SetValue{AltText}{%



}\SetValue{Solution}{%

Step 1: Use logarithmic identities

We can use the identity:

$$
\ln \dfrac{n}{n+1}=\ln n-\ln (n+1)
$$


So the series becomes:

$$
\sum_{n=1}^{\infty}(\ln n-\ln (n+1))
$$


Step 2: Write as a telescoping sum

This is a telescoping series:

$$
(\ln 1-\ln 2)+(\ln 2-\ln 3)+(\ln 3-\ln 4)+\cdots
$$


You can see that terms cancel in sequence:

- $\ln 1$ stays

- $-\ln 2+\ln 2=0$

- $-\ln 3+\ln 3=0$

- ...

- Only $\ln 1$ and $-\ln (n+1)$ remain in the $n$-th partial sum

So the partial sum is:

$$
s_N=\ln 1-\ln (N+1)=0-\ln (N+1)=-\ln (N+1)
$$


Step 3: Take the limit

$$
\lim _{N \rightarrow \infty} s_N=\lim _{N \rightarrow \infty}-\ln (N+1)=-\infty
$$

Final Answer:

- The series diverges.

- In fact, it diverges to $-\infty$.

The series diverges (to $-\infty$).

}\SetValue{Rubric}{%Markdown



}\SetValue{Hint}{%
Solution Goes Here
}\SetValue{Answer}{%

}
\ProcessDATA



