\SetValue{Module}{1}\SetValue{SectionAB}{A}\SetValue{MainChapter}{}\SetValue{SubChapter}{}\SetValue{Contents}{%%
    
Determine whether the series is convergent or divergent by expressing $s_n$ as a telescoping sum. If it is convergent, find its sum.

$$\sum_{n=1}^{\infty}\left(e^{1 / n}-e^{1 /(n-1)}\right)$$

}\SetValue{Concept}{%



}\SetValue{AltText}{%



}\SetValue{Solution}{%

Step 1: Understanding the Terms

We can write the first few terms of the series:

- For $n=1: e^{1 / 1}-e^{1 / 0}=e-e^{\infty}$

But $e^{1 / 0}$ is undefined, so the term is not defined at $n=1$.

Thus, we need to re-index the sum to avoid the undefined term.

Let's shift the index to start at $n=2$ :

$$
\sum_{n=2}^{\infty}\left(e^{1 / n}-e^{1 /(n-1)}\right)
$$

Step 2: Write as a Telescoping Sum

Let's write out the partial sums:

$$
s_N=\sum_{n=2}^N\left(e^{1 / n}-e^{1 /(n-1)}\right)
$$


Write a few terms explicitly:

$$
=\left(e^{1 / 2}-e^{1 / 1}\right)+\left(e^{1 / 3}-e^{1 / 2}\right)+\left(e^{1 / 4}-e^{1 / 3}\right)+\cdots+\left(e^{1 / N}-e^{1 /(N-1)}\right)
$$


Observe the telescoping cancellation:

- $e^{1 / 2}$ cancels with $-e^{1 / 2}$,

- $e^{1 / 3}$ cancels with $-e^{1 / 3}$,

- ...

- The only terms not canceled are:

$$
-e^{1 / 1}=-e \quad \text { and } \quad+e^{1 / N}
$$


Thus, the partial sum is:

$$
s_N=e^{1 / N}-e
$$

Step 3: Take the Limit of the Partial Sum

To determine convergence, compute the limit of $s_N$ as $N \rightarrow \infty$:

$$
\lim _{N \rightarrow \infty} s_N=\lim _{N \rightarrow \infty}\left(e^{1 / N}-e\right)=1-e
$$


Therefore, the series converges, and the sum is:

$$
1-e
$$

}\SetValue{Rubric}{%Markdown



}\SetValue{Hint}{%
Solution Goes Here
}\SetValue{Answer}{%

}
\ProcessDATA



