\SetValue{Module}{1}\SetValue{SectionAB}{A}\SetValue{MainChapter}{}\SetValue{SubChapter}{}\SetValue{Contents}{%%
    
Find the values of $x$ for which the series converges. Find the sum of the series for those values of $x$.

$$\sum_{n=1}^{\infty}(-5)^n x^n$$

}\SetValue{Concept}{%



}\SetValue{AltText}{%



}\SetValue{Solution}{%

Step 1: Recognize the Series Type

This is a geometric series of the form:

$$
\sum_{n=1}^{\infty} a r^n
$$


Here,

- $a=-5 x$ (first term when $n=1$ ),

- common ratio $r=-5 x$

So we can write:

$$
\sum_{n=1}^{\infty}(-5 x)^n=(-5 x)+(-5 x)^2+(-5 x)^3+\cdots
$$


Step 2: Convergence Condition

A geometric series $\sum_{n=0}^{\infty} r^n$ converges if and only if:

$$
|r|<1
$$


In our case, the ratio is $r=-5 x$, so the convergence condition is:

$$
|-5 x|<1 \quad \Rightarrow \quad|x|<\dfrac{1}{5}
$$

Step 3: Find the Sum

Let's first recall the sum formula for a geometric series starting at $n=0$ :

$$
\sum_{n=0}^{\infty} r^n=\dfrac{1}{1-r}
$$


But our series starts at $n=1$, so we subtract the $n=0$ term:

$$
\sum_{n=1}^{\infty} r^n=\dfrac{r}{1-r}
$$


Substitute $r=-5 x$ :

$$
\sum_{n=1}^{\infty}(-5 x)^n=\dfrac{-5 x}{1-(-5 x)}=\dfrac{-5 x}{1+5 x}
$$

Final Answer:

- The series converges for:

$$
|x|<\dfrac{1}{5}
$$

- For those values of $x$, the sum is:

$$
\dfrac{-5 x}{1+5 x}
$$


}\SetValue{Rubric}{%Markdown



}\SetValue{Hint}{%
Solution Goes Here
}\SetValue{Answer}{%

}
\ProcessDATA



