\SetValue{Module}{1}\SetValue{SectionAB}{A}\SetValue{MainChapter}{}\SetValue{SubChapter}{}\SetValue{Contents}{%%
    
Find the values of $x$ for which the series converges. Find the sum of the series for those values of $x$.

$$\sum_{n=1}^{\infty}(x+2)^n$$

}\SetValue{Concept}{%



}\SetValue{AltText}{%



}\SetValue{Solution}{%

Step 1: Recognize the Series Type

This is a geometric series of the form:

$$
\sum_{n=1}^{\infty} r^n
$$

with common ratio $r=x+2$.

Step 2: Convergence Condition

A geometric series $\sum_{n=1}^{\infty} r^n$ converges if and only if:

$$
|r|<1
$$


So in our case:

$$
|x+2|<1
$$


Solve this inequality:

$$
-1<x+2<1
$$


Subtract 2 from all sides:

$$
-3<x<-1
$$

So the series converges for:

$$
-3<x<-1
$$

Step 3: Find the Sum

The sum of a geometric series starting at $n=1$ is:

$$
\sum_{n=1}^{\infty} r^n=\dfrac{r}{1-r}
$$


Here, $r=x+2$, so:

$$
\sum_{n=1}^{\infty}(x+2)^n=\dfrac{x+2}{1-(x+2)}=\dfrac{x+2}{-x-1}
$$


You can simplify:

$$
\dfrac{x+2}{-x-1}=-1 \cdot \dfrac{x+2}{x+1}
$$


Final Answer:

- The series converges for:

$$
-3<x<-1
$$

- For those values of $x$, the sum is:

$$
\dfrac{x+2}{-x-1}
$$

}\SetValue{Rubric}{%Markdown



}\SetValue{Hint}{%
Solution Goes Here
}\SetValue{Answer}{%

}
\ProcessDATA



