\SetValue{Module}{1}\SetValue{SectionAB}{A}\SetValue{MainChapter}{}\SetValue{SubChapter}{}\SetValue{Contents}{%%
    
Find the values of $x$ for which the series converges. Find the sum of the series for those values of $x$.

$$\sum_{n=0}^{\infty} \dfrac{(x-2)^n}{3^n}$$

}\SetValue{Concept}{%



}\SetValue{AltText}{%



}\SetValue{Solution}{%

Step 1: Recognize the Series Type

This is a geometric series:

$$
\sum_{n=0}^{\infty}\left(\dfrac{x-2}{3}\right)^n
$$


Let:

$$
r=\dfrac{x-2}{3}
$$

Step 2: Convergence Condition

A geometric series $\sum r^n$ (starting from $n=0$ ) converges if and only if:

$$
|r|<1
$$


So:

$$
\left|\dfrac{x-2}{3}\right|<1
$$


Multiply both sides by 3:

$$
|x-2|<3
$$


This gives the interval of convergence:

$$
-3<x-2<3 \quad \Rightarrow \quad-1<x<5
$$


So the series converges for:

$$
-1<x<5
$$

Step 3: Find the Sum

The sum of a geometric series $\sum_{n=0}^{\infty} r^n$ is:

$$
\dfrac{1}{1-r}
$$


In this case, $r=\dfrac{x-2}{3}$, so the sum is:

$$
\sum_{n=0}^{\infty}\left(\dfrac{x-2}{3}\right)^n=\dfrac{1}{1-\dfrac{x-2}{3}}=\dfrac{1}{\dfrac{3-(x-2)}{3}}=\dfrac{3}{5-x}
$$

Final Answer:

- The series converges for:

$$
-1<x<5
$$

- For those values of $x$, the sum is:

$$
\dfrac{3}{5-x}
$$


}\SetValue{Rubric}{%Markdown



}\SetValue{Hint}{%
Solution Goes Here
}\SetValue{Answer}{%

}
\ProcessDATA



