\SetValue{Module}{1}\SetValue{SectionAB}{A}\SetValue{MainChapter}{}\SetValue{SubChapter}{}\SetValue{Contents}{%%
    
Find the values of $x$ for which the series converges. Find the sum of the series for those values of $x$.

$$\sum_{n=0}^{\infty}(-4)^n(x-5)^n$$

}\SetValue{Concept}{%



}\SetValue{AltText}{%



}\SetValue{Solution}{%

Step 1: Recognize the Series Type

This is a geometric series of the form:

$$
\sum_{n=0}^{\infty} r^n \quad \text { with } \quad r=(-4)(x-5)
$$


So the general term is:

$$
[(-4)(x-5)]^n
$$


Let's define:

$$
r=-4(x-5)
$$


Step 2: Convergence Condition

A geometric series $\sum r^n$ converges if and only if:

$$
|r|<1
$$


So:

$$
|-4(x-5)|<1 \quad \Rightarrow \quad|x-5|<\dfrac{1}{4}
$$


This gives the interval:

$$
\dfrac{19}{4}<x<\dfrac{21}{4}
$$

Step 3: Find the Sum

The sum of a geometric series $\sum_{n=0}^{\infty} r^n$ is:

$$
\dfrac{1}{1-r}
$$


Substitute $r=-4(x-5)$:

$$
\sum_{n=0}^{\infty}(-4)^n(x-5)^n=\dfrac{1}{1+4(x-5)}=\dfrac{1}{4 x-19}
$$

Final Answer:

- The series converges for:

$$
\dfrac{19}{4}<x<\dfrac{21}{4}
$$

- For those values of $x$, the sum is: $4 x-19$

}\SetValue{Rubric}{%Markdown



}\SetValue{Hint}{%
Solution Goes Here
}\SetValue{Answer}{%

}
\ProcessDATA



