\SetValue{SectionAB}{}\SetValue{MainChapter}{}\SetValue{SubChapter}{}\SetValue{Contents}{%

$$ \sqrt{-6 x+6}+2=x+1 $$ What is the solution set of the equation above? 

\ansFOURs{%start
	\{-1\}   }{%<--- (A)
	\{1\}   }{%<--- (B)
	\{-1,-5\}   }{%<--- (C)
    \{1,-5\} }%<---- (D)

}\SetValue{Solution}{%

We need to find the solution set for the equation \( \sqrt{-6x + 6} + 2 = x + 1 \).

\begin{alignat*}{2}
\sqrt{-6x + 6} + 2 &= x + 1 \qquad && \{ \text{Given equation} \} \\
\sqrt{-6x + 6} &= x - 1 \qquad && \{ \text{Subtract 2 from both sides} \} \\
\left(\sqrt{-6x + 6}\right)^2 &= (x - 1)^2 \qquad && \{ \text{Square both sides} \} \\
-6x + 6 &= x^2 - 2x + 1 \qquad && \{ \text{Expand the right side} \} \\
0 &= x^2 + 4x - 5 \qquad && \{ \text{Move all terms to one side} \}
\end{alignat*}

Now, we will solve the quadratic equation.

\begin{alignat*}{2}
(x + 5)(x - 1) &= 0 \qquad && \{ \text{Factor the quadratic} \} \\
x &= -5, \, 1 \qquad && \{ \text{Solve for } x \}
\end{alignat*}

Check each solution in the original equation.

Checking \( x = -5 \):
\[
\sqrt{-6(-5) + 6} + 2 = -5 + 1
\]
\[
\sqrt{36} + 2 = -4 \Rightarrow 6 + 2 = -4 \quad \text{(False)}
\]

Checking \( x = 1 \):
\[
\sqrt{-6(1) + 6} + 2 = 1 + 1
\]
\[
\sqrt{0} + 2 = 2 \Rightarrow 0 + 2 = 2 \quad \text{(True)}
\]

The only valid solution is \( x = 1 \).

Thus, the correct answer is $\fbox{B) $1$}$.

}\SetValue{Answer}{%
C
}
\ProcessDATA


