\SetValue{SectionAB}{}\SetValue{MainChapter}{}\SetValue{SubChapter}{}\SetValue{Contents}{%
  
\begin{align*} \frac{x^2+x-2}{x-1} = \sqrt{2x+7} 
\end{align*} 
For the equation above, there are two potential solutions. However, one of them is extraneous. What is the value of the extraneous solution? 

\ansFOURs{%start
1}{%<--- (A) 
2}{%<--- (B) 
3}{%<--- (C) 
-1}%<---- (D)

}\SetValue{Solution}{%

Given the equation:
\[
\frac{x^2 + x - 2}{x - 1} = \sqrt{2x + 7}
\]
we need to find the extraneous solution by simplifying and solving.

### Step 1: Simplify the Left Side

First, factor the numerator \(x^2 + x - 2\) as:
\[
x^2 + x - 2 = (x - 1)(x + 2)
\]
Then, the expression becomes:
\[
\frac{(x - 1)(x + 2)}{x - 1}
\]
For \(x \neq 1\), this simplifies to \(x + 2\).

### Step 2: Solve the Equation

The equation now is:
\[
x + 2 = \sqrt{2x + 7}
\]
Square both sides to get rid of the square root:
\[
(x + 2)^2 = 2x + 7
\]
Expanding the left side:
\[
x^2 + 4x + 4 = 2x + 7
\]

### Step 3: Move All Terms to One Side

Subtract \(2x + 7\) from both sides:
\[
x^2 + 2x - 3 = 0
\]

### Step 4: Factor the Quadratic

\[
x^2 + 2x - 3 = (x - 1)(x + 3) = 0
\]

### Step 5: Solve for \(x\)

The solutions are:
\[
x = 1 \quad \text{and} \quad x = -3
\]

### Step 6: Check for Extraneous Solutions
For \(x = 1\):
\[
\frac{1^2 + 1 - 2}{1 - 1} = \frac{0}{0} \quad \text{(undefined)}
\]
So, \(x = 1\) is extraneous.

For \(x = -3\):
\[
\frac{(-3)^2 + (-3) - 2}{-3 - 1} = \frac{4}{-4} = -1
\]
\[
\sqrt{2(-3) + 7} = \sqrt{1} = 1
\]
Since \(-1 \neq 1\), this does not satisfy the original equation.

Thus, the extraneous solution is $\fbox{A) $1$}$.

}\SetValue{Answer}{%
D
}
\ProcessDATA

