\SetValue{SectionAB}{}\SetValue{MainChapter}{}\SetValue{SubChapter}{}\SetValue{Contents}{%

If \( a^{-\tfrac{2}{3}} = x \), where \( a > 0 \), which of the following is NOT equal to \( a \) in terms of \( x \)? 

\ansFOURsT{ 
\( \frac{1}{x\sqrt{x}} \)}{%<--- (A) 
\( \left(\frac{1}{x}\right)^{\tfrac{3}{2}} \)}{%<--- (B) 
\( x^{-\tfrac{3}{2}} \)}{%<--- (C) 
\( \left(\frac{1}{x}\right)^{\tfrac{2}{3}} \)}%<---- (D)

}\SetValue{Solution}{%

We start by solving for \( a \) in terms of \( x \) using the given equation \( a^{-\tfrac{2}{3}} = x \).

\begin{alignat*}{3}
a^{-\tfrac{2}{3}} &= x \qquad && \{ \text{Given} \} \\
a &= x^{-\tfrac{3}{2}} \qquad && \{ \text{Raise both sides to the power of } -\frac{3}{2} \}
\end{alignat*}

Now, let's analyze each option to determine which one is NOT equal to \( a = x^{-\tfrac{3}{2}} \).

%\begin{enumerate}[label={\textbf{(\Alph*)}}]
1. \( \frac{1}{x \sqrt{x}} \): **True**. 
\[
\frac{1}{x \sqrt{x}} = \frac{1}{x \cdot x^{\tfrac{1}{2}}} = \frac{1}{x^{\tfrac{3}{2}}} = x^{-\tfrac{3}{2}}
\]
This is equal to \( a \).

2. \( \left(\frac{1}{x}\right)^{\tfrac{3}{2}} \): **True**. 
\[
\left(\frac{1}{x}\right)^{\tfrac{3}{2}} = \frac{1}{x^{\tfrac{3}{2}}} = x^{-\tfrac{3}{2}}
\]
This is also equal to \( a \).

3. \( x^{-\tfrac{3}{2}} \): **True**. 
This is exactly equal to \( a \).

4. \( \left(\frac{1}{x}\right)^{\tfrac{2}{3}} \):  **False**. 
\[
\left(\frac{1}{x}\right)^{\tfrac{2}{3}} = \frac{1}{x^{\tfrac{2}{3}}}
\]
This is not equal to \( x^{-\tfrac{3}{2}} \), so this is not equal to \( a \).
%\end{enumerate}

The expression that is NOT equal to \( a \) is: $\fbox{D) $\left(\frac{1}{x}\right)^{\tfrac{2}{3}}$}$



}\SetValue{Answer}{%
3/4
}
\ProcessDATA


