\SetValue{SectionAB}{}\SetValue{MainChapter}{}\SetValue{SubChapter}{}\SetValue{Contents}{%

$$ 2 i(4-3 i)\left(2+\frac{3}{2} i\right) $$ Which of the following complex numbers is equivalent to the expression above? (Note: $i=\sqrt{-1}$ ) 

\ansFOURs{%start
	  18-24 i}{%<--- (A)
	  24+18 i}{%<--- (B)
	  16 i}{%<--- (C)
	  25 i}%<---- (D)
	  
}\SetValue{Solution}{%

First, we start by simplifying the expression \( 2i(4-3i) \left( 2 + \frac{3}{2} i \right) \). We will break this down into smaller steps.

\begin{alignat*}{2}
2i(4 - 3i) &= 2i \cdot 4 + 2i \cdot (-3i) \qquad && \{\text{Distribute $2i$}  \} \\
&= 8i - 6i^2 \qquad && \{ \text{Simplifying each term} \} \\
&= 8i + 6 \qquad && \{ \text{Substitute $i^2 = -1$} \} \\
\end{alignat*}

Now, we multiply the result \( 8i + 6 \) by \( \left( 2 + \frac{3}{2} i \right) \).

\begin{alignat*}{2}
(8i + 6)\left( 2 + \frac{3}{2} i \right) &= 8i \cdot 2 + 8i \cdot \frac{3}{2}i + 6 \cdot 2 + 6 \cdot \frac{3}{2}i \qquad && \{\text{ Distribute  terms}\} \\
&= 16i + 12i^2 + 12 + 9i \qquad && \{ \text{Simplify each product} \} \\
&= 16i - 12 + 12 + 9i \qquad && \{ \text{Substitute $i^2 = -1$} \} \\
&= 25i \qquad && \{ \text{Combine like terms} \} \\
\end{alignat*}

The final expression simplifies to $\fbox{D) $25i$}$.



}\SetValue{Answer}{%
13/4
}
\ProcessDATA


