\SetValue{SectionAB}{}\SetValue{MainChapter}{}\SetValue{SubChapter}{}\SetValue{Contents}{%

Evaluate the integral.

$$\int \dfrac{x^3}{\sqrt{x^2+4}}\  d x $$

}\SetValue{Solution}{%

Step 1: Use substitution

Let's use the substitution:

$$
u=x^2+4 \Rightarrow d u=2 x d x
$$


We can write $x^3=x \cdot x^2=x(u-4)$, and since $x d x=\dfrac{1}{2} d u$, we get:

$$
\int \dfrac{x^3}{\sqrt{x^2+4}} d x=\int \dfrac{x(u-4)}{\sqrt{u}} \cdot d x
$$


Now use $x d x=\dfrac{1}{2} d u$ :

$$
=\int \dfrac{(u-4)}{\sqrt{u}} \cdot \dfrac{1}{2} d u=\dfrac{1}{2} \int \dfrac{u-4}{\sqrt{u}} d u
$$


Step 2: Simplify the integrand

$$
\dfrac{u-4}{\sqrt{u}}=\dfrac{u}{\sqrt{u}}-\dfrac{4}{\sqrt{u}}=u^{1 / 2}-4 u^{-1 / 2}
$$


So the integral becomes:

$$
\dfrac{1}{2} \int\left(u^{1 / 2}-4 u^{-1 / 2}\right) d u
$$


Step 3: Integrate term by term

$$
\dfrac{1}{2}\left(\dfrac{2}{3} u^{3 / 2}-8 u^{1 / 2}\right)+C=\dfrac{1}{3} u^{3 / 2}-4 u^{1 / 2}+C
$$


Step 4: Back-substitute $u=x^2+4$

$$
=\dfrac{1}{3}\left(x^2+4\right)^{3 / 2}-4\left(x^2+4\right)^{1 / 2}+C
$$


Final Answer:

$$
\dfrac{1}{3}\left(x^2+4\right)^{3 / 2}-4\left(x^2+4\right)^{\frac{1}{2}}+C
$$

}\SetValue{Rubric}{%

# General Scoring Notes


## Model Solution (a)


## Scoring (a)

For $\text { Area }=\int_0^2(f(x)-g(x)) d x$,
Integrand; 1 point, Answer; 1 point.

## Scoring notes (a)


}\SetValue{Answer}{%

$\dfrac{1}{3}\left(x^2+4\right)^{\frac{3}{2}}-4\left(x^2+4\right)^{\frac{1}{2}}+C$

}
\ProcessDATA

