\SetValue{SectionAB}{}\SetValue{MainChapter}{}\SetValue{SubChapter}{}\SetValue{Contents}{%

Evaluate the integral.

$$\int_0^3 \dfrac{x}{\sqrt{36-x^2}}\  d x$$

}\SetValue{Solution}{%

We want to evaluate

$$
\int_0^3 \dfrac{x}{\sqrt{36-x^2}} d x
$$


A straightforward method is to use the substitution $u=36-x^2$.

Step 1: Substitution
Let

$$
u=36-x^2 \quad \Longrightarrow \quad d u=-2 x d x \quad \Longrightarrow \quad x d x=-\dfrac{1}{2} d u.
$$


When $x=0, u=36-0^2=36$.
When $x=3, u=36-3^2=36-9=27$.
Thus the integral becomes

$$
\int_0^3 \dfrac{x}{\sqrt{36-x^2}} d x=\int_{x=0}^{x=3} \dfrac{x}{\sqrt{u}}\left(-\dfrac{1}{2} d u\right)=-\dfrac{1}{2} \int_{u=36}^{u=27} \dfrac{1}{\sqrt{u}} d u.
$$

Step 2: Reverse the limits to remove the minus sign
We have

$$
-\dfrac{1}{2} \int_{u=36}^{u=27} u^{-\dfrac{1}{2}} d u=\dfrac{1}{2} \int_{u=27}^{u=36} u^{-\dfrac{1}{2}} d u
$$


Step 3: Integrate $u^{-1 / 2}$

$$
\int u^{-1 / 2} d u=2 \sqrt{u}
$$


Thus,

$$
\dfrac{1}{2} \int_{27}^{36} u^{-1 / 2} d u=\dfrac{1}{2}[2 \sqrt{u}]_{27}^{36}=[\sqrt{u}]_{27}^{36}=\sqrt{36}-\sqrt{27}=6-3 \sqrt{3}.
$$


Hence the definite integral is

$$
\int_0^3 \dfrac{x}{\sqrt{36-x^2}} d x=6-3 \sqrt{3}
$$

}\SetValue{Rubric}{%

# General Scoring Notes


## Model Solution (a)


## Scoring (a)

For $\text { Area }=\int_0^2(f(x)-g(x)) d x$,
Integrand; 1 point, Answer; 1 point.

## Scoring notes (a)


}\SetValue{Answer}{%

}
\ProcessDATA

