\SetValue{SectionAB}{}\SetValue{MainChapter}{}\SetValue{SubChapter}{}\SetValue{Contents}{%

Solve for $x$ in the equation below:

$$
7+2(x-3)=-3(x+1)-4
$$

\ansFOURs{%start
-\frac{8}{5}}{%<--- (A)
 -1}{%<--- (B)
-\frac{8}{3}}{%<--- (C)
 3}%<---- (D)
}\SetValue{Solution}{%

Answer: \textbf{(A)}

Let's solve for $x$ in the given equation:

$
7 + 2(x - 3) = -3(x + 1) - 4
$

 Step 1: Distribute
Expanding both sides:

$
7 + 2x - 6 = -3x - 3 - 4
$

Simplify:

$
1 + 2x = -3x - 7
$

 Step 2: Move Terms
Add $3x$ to both sides:

$
1 + 5x = -7
$

Subtract 1 from both sides:

$
5x = -8
$

 Step 3: Solve for $x$
$
x = \frac{-8}{5}
$

 Step 4: Select the Correct Answer
The correct choice is $A) -\frac{8}{5}$.


}\SetValue{Answer}{%
A
}
\ProcessDATA


