\SetValue{SectionAB}{}\SetValue{MainChapter}{}\SetValue{SubChapter}{}\SetValue{Contents}{%

Evaluate the integral.

$$\int\ t\ e^{-3t}\ d t$$

}\SetValue{Solution}{%

To integrate

$$
\int t e^{-3 t} d t
$$

we use integration by parts. Let

$$
u=t \quad \text { and } \quad d v=e^{-3 t} d t
$$


Then

$$
d u=d t \quad \text { and } \quad v=\int e^{-3 t} d t=-\dfrac{1}{3} e^{-3 t}
$$


Applying the integration by parts formula

$$
\int u d v=u v-\int v d u
$$

we get

$$
\int t e^{-3 t} d t=t \cdot\left(-\dfrac{1}{3} e^{-3 t}\right)-\int\left(-\dfrac{1}{3} e^{-3 t}\right) d t
$$


Simplify step by step:
1. First part:

$$
t \cdot\left(-\dfrac{1}{3} e^{-3 t}\right)=-\dfrac{t}{3} e^{-3 t}
$$

2. Second part:

$$
-\int\left(-\dfrac{1}{3} e^{-3 t}\right) d t=\dfrac{1}{3} \int e^{-3 t} d t=\dfrac{1}{3}\left(-\dfrac{1}{3}\right) e^{-3 t}=-\dfrac{1}{9} e^{-3 t}
$$


Combine the two parts:

$$
\int t e^{-3 t} d t=-\dfrac{t}{3} e^{-3 t}-\dfrac{1}{9} e^{-3 t}+C
$$


You can also factor out $-\dfrac{1}{3} e^{-3 t}$ :

$$
\int t e^{-3 t} d t=-\dfrac{1}{3} e^{-3 t}\left(t+\dfrac{1}{3}\right)+C
$$

where $C$ is the constant of integration.

}\SetValue{Rubric}{%




}\SetValue{Answer}{%

}
\ProcessDATA



   
   
   

   


