\SetValue{SectionAB}{}\SetValue{MainChapter}{}\SetValue{SubChapter}{}\SetValue{Contents}{%

Evaluate the integral.

$$\int\ (x^2+2x)\ \cos \ x\ d x$$

}\SetValue{Solution}{%

We want to evaluate

$$
\int\left(x^2+2 x\right) \cos (x) d x
$$


A straightforward way is to split it and integrate each part:

$$
\int\left(x^2+2 x\right) \cos (x) d x=\int x^2 \cos (x) d x+2 \int x \cos (x) d x
$$


We'll handle these two integrals one at a time.
1) The integral $\int x^2 \cos (x) d x$

Use integration by parts. Let

$$
u=x^2 \quad \text { and } \quad d v=\cos (x) d x
$$


Then

$$
d u=2 x d x \quad \text { and } \quad v=\sin (x)
$$


By the formula $\int u d v=u v-\int v d u$,

$$
\int x^2 \cos (x) d x=x^2 \sin (x)-\int \sin (x)(2 x d x)
$$


So

$$
\int x^2 \cos (x) d x=x^2 \sin (x)-2 \int x \sin (x) d x
$$


We must now handle $\int x \sin (x) d x$ again by parts:
- Let $u=x$ and $d v=\sin (x) d x$.
- Then $d u=d x$ and $v=-\cos (x)$.

Hence,

$$
\int x \sin (x) d x=x(-\cos (x))-\int(-\cos (x)) d x=-x \cos (x)+\int \cos (x) d x=-x \cos (x)+\sin (x)
$$


Therefore,

$$
2 \int x \sin (x) d x=2[-x \cos (x)+\sin (x)]=-2 x \cos (x)+2 \sin (x) .
$$


Substitute back:

$$
\int x^2 \cos (x) d x=x^2 \sin (x)-[-2 x \cos (x)+2 \sin (x)]=x^2 \sin (x)+2 x \cos (x)-2 \sin (x)
$$

2) The integral $\int x \cos (x) d x$

Again, integration by parts:
- Let $u=x, d v=\cos (x) d x$.
- Then $d u=d x, v=\sin (x)$.

So

$$
\int x \cos (x) d x=x \sin (x)-\int \sin (x) d x=x \sin (x)+\cos (x)
$$

3) Combine the results

We had

$$
\int\left(x^2+2 x\right) \cos (x) d x=\int x^2 \cos (x) d x+2 \int x \cos (x) d x
$$


Substitute our two findings:
1. $\int x^2 \cos (x) d x=x^2 \sin (x)+2 x \cos (x)-2 \sin (x)$.
2. $\int x \cos (x) d x=x \sin (x)+\cos (x)$.

Thus,

$$
\int\left(x^2+2 x\right) \cos (x) d x=\left[x^2 \sin (x)+2 x \cos (x)-2 \sin (x)\right]+2[x \sin (x)+\cos (x)]
$$


Distribute the 2 in the second bracket:

$$
=x^2 \sin (x)+2 x \cos (x)-2 \sin (x)+2 x \sin (x)+2 \cos (x)
$$


Combine like terms in a tidy way, for instance grouping $\sin (x)$ terms and $\cos (x)$ terms:

- The $\sin (x)$ terms:

$$
x^2 \sin (x)+2 x \sin (x)-2 \sin (x)=\sin (x)\left(x^2+2 x-2\right)
$$

- The $\cos (x)$ terms:

$$
2 x \cos (x)+2 \cos (x)=2 \cos (x)(x+1)
$$


A nice factored form is therefore

$$
\int\left(x^2+2 x\right) \cos (x) d x=\sin (x)\left(x^2+2 x-2\right)+2 \cos (x)(x+1)+C
$$


Either that, or you can leave it un-factored if you prefer. Both forms are correct.
Including the constant of integration $C$, the final answer is:

$$
\int\left(x^2+2 x\right) \cos (x) d x=x^2 \sin (x)+2 x \cos (x)-2 \sin (x)+2 x \sin (x)+2 \cos (x)+C
$$


Or in the factored version:

$$
\int\left(x^2+2 x\right) \cos (x) d x=\sin (x)\left(x^2+2 x-2\right)+2 \cos (x)(x+1)+C.
$$

}\SetValue{Rubric}{%




}\SetValue{Answer}{%

}
\ProcessDATA



   
   

   


