\SetValue{SectionAB}{}\SetValue{MainChapter}{}\SetValue{SubChapter}{}\SetValue{Contents}{%

Evaluate the integral.

$$\int\ t^2\ \sin \ \beta \ t\ d t$$

}\SetValue{Solution}{%

We want to evaluate

$$
\int t^2 \sin (\beta t) d t
$$

where $\beta$ is a constant.

Step 1: First integration by parts
Choose:

$$
u=t^2, \quad d v=\sin (\beta t) d t
$$


Then

$$
d u=2 t d t, \quad v=\int \sin (\beta t) d t=-\dfrac{1}{\beta} \cos (\beta t)
$$


By the integration by parts formula,

$$
\int u d v=u v-\int v d u
$$

we get:

$$
\int t^2 \sin (\beta t) d t=t^2\left(-\dfrac{1}{\beta} \cos (\beta t)\right)-\int\left(-\dfrac{1}{\beta} \cos (\beta t)\right)(2 t d t)
$$


Simplify step by step:

1. The first term is

$$
t^2 \cdot\left(-\dfrac{1}{\beta}\right) \cos (\beta t)=-\dfrac{t^2}{\beta} \cos (\beta t)
$$

2. The second term becomes

$$
-\int\left(-\dfrac{1}{\beta}\right) \cos (\beta t)(2 t) d t=+\dfrac{2}{\beta} \int t \cos (\beta t) d t
$$


So

$$
\int t^2 \sin (\beta t) d t=-\dfrac{t^2}{\beta} \cos (\beta t)+\dfrac{2}{\beta} \int t \cos (\beta t) d t
$$


Step 2: Second integration by parts for $\int t \cos (\beta t) d t$
Choose:

$$
u=t, \quad d v=\cos (\beta t) d t
$$


Then

$$
d u=d t, \quad v=\int \cos (\beta t) d t=\dfrac{1}{\beta} \sin (\beta t)
$$


Apply integration by parts again:

$$
\int t \cos (\beta t) d t=t \cdot\left(\dfrac{1}{\beta} \sin (\beta t)\right)-\int\left(\dfrac{1}{\beta} \sin (\beta t)\right)(d t)
$$


That is

$$
\int t \cos (\beta t) d t=\dfrac{t}{\beta} \sin (\beta t)-\dfrac{1}{\beta} \int \sin (\beta t) d t
$$


We know

$$
\int \sin (\beta t) d t=-\dfrac{1}{\beta} \cos (\beta t)
$$


Hence

$$
-\dfrac{1}{\beta} \int \sin (\beta t) d t=-\dfrac{1}{\beta}\left(-\dfrac{1}{\beta} \cos (\beta t)\right)=+\dfrac{1}{\beta^2} \cos (\beta t) .
$$


So

$$
\int t \cos (\beta t) d t=\dfrac{t}{\beta} \sin (\beta t)+\dfrac{1}{\beta^2} \cos (\beta t)
$$


Step 3: Combine both parts
Returning to our expression:

$$
\int t^2 \sin (\beta t) d t=-\dfrac{t^2}{\beta} \cos (\beta t)+\dfrac{2}{\beta} \int t \cos (\beta t) d t
$$

We have just found:

$$
\int t \cos (\beta t) d t=\dfrac{t}{\beta} \sin (\beta t)+\dfrac{1}{\beta^2} \cos (\beta t)
$$


Hence

$$
\dfrac{2}{\beta} \int t \cos (\beta t) d t=\dfrac{2}{\beta}\left(\dfrac{t}{\beta} \sin (\beta t)+\dfrac{1}{\beta^2} \cos (\beta t)\right)=\dfrac{2 t}{\beta^2} \sin (\beta t)+\dfrac{2}{\beta^3} \cos (\beta t) .
$$


Putting it all together:

$$
\int t^2 \sin (\beta t) d t=-\dfrac{t^2}{\beta} \cos (\beta t)+\dfrac{2 t}{\beta^2} \sin (\beta t)+\dfrac{2}{\beta^3} \cos (\beta t)+C
$$

where $C$ is the constant of integration.

Final Answer

$$
\int t^2 \sin (\beta t) d t=-\dfrac{t^2}{\beta} \cos (\beta t)+\dfrac{2 t}{\beta^2} \sin (\beta t)+\dfrac{2}{\beta^3} \cos (\beta t)+C
$$

}\SetValue{Rubric}{%




}\SetValue{Answer}{%

}
\ProcessDATA



   
   

   


