\SetValue{SectionAB}{}\SetValue{MainChapter}{}\SetValue{SubChapter}{}\SetValue{Contents}{%

Evaluate the integral.

$$\int\ s\ 2^s\ d s$$

}\SetValue{Solution}{%

We want to evaluate

$$
\int s 2^s d s
$$


A convenient method is integration by parts. Recall the formula:

$$
\int u d v=u v-\int v d u
$$


Step 1: Choose $u$ and $d v$
Let

$$
u=s, \quad d v=2^s d s
$$


Then,

$$
d u=d s, \quad v=\int 2^s d s
$$


To find $v$, recall that $2^s=e^{(\ln 2) s}$. Thus,

$$
\int 2^s d s=\int e^{(\ln 2) s} d s=\dfrac{1}{\ln 2} e^{(\ln 2) s}=\dfrac{2^s}{\ln 2}
$$


Hence,

$$
v=\dfrac{2^s}{\ln 2}
$$

Step 2: Apply the integration by parts formula

$$
\int s 2^s d s=u v-\int v d u=s\left(\dfrac{2^s}{\ln 2}\right)-\int \dfrac{2^s}{\ln 2}(d s) .
$$


Factor out $\dfrac{1}{\ln 2}$ where it is convenient:

$$
=\dfrac{s 2^s}{\ln 2}-\dfrac{1}{\ln 2} \int 2^s d s
$$


Step 3: Integrate $\int 2^s d s$
As before,

$$
\int 2^s d s=\dfrac{2^s}{\ln 2}
$$


Thus,

$$
-\dfrac{1}{\ln 2} \int 2^s d s=-\dfrac{1}{\ln 2}\left(\dfrac{2^s}{\ln 2}\right)=-\dfrac{2^s}{(\ln 2)^2} .
$$

Step 4: Combine everything
Putting it all together:

$$
\int s 2^s d s=\dfrac{s 2^s}{\ln 2}-\dfrac{2^s}{(\ln 2)^2}+C
$$

where $C$ is the constant of integration.

Final Answer

$$
\int s 2^s d s=\dfrac{s 2^s}{\ln 2}-\dfrac{2^s}{(\ln 2)^2}+C.
$$

}\SetValue{Rubric}{%




}\SetValue{Answer}{%

}
\ProcessDATA


 
   
   

   


