\SetValue{SectionAB}{}\SetValue{MainChapter}{}\SetValue{SubChapter}{}\SetValue{Contents}{%

Evaluate the integral.

$$\int\ \left( \ln\ x \right)^2 \ d x$$

}\SetValue{Solution}{%

We want to evaluate

$$
\int(\ln x)^2 d x
$$


A natural approach is integration by parts. Recall:

$$
\int u d v=u v-\int v d u .
$$


Step 1: Choose $u$ and $d v$
Set

$$
u=(\ln x)^2, \quad d v=d x
$$


Then

$$
d u=2(\ln x) \frac{1}{x} d x=\frac{2 \ln x}{x} d x, \quad v=\int 1 d x=x .
$$

Step 2: Apply the integration by parts formula

$$
\begin{aligned}
\int(\ln x)^2 d x & =\underbrace{(\ln x)^2}_u \cdot \underbrace{x}_v-\int \underbrace{x}_v \cdot \underbrace{\frac{2 \ln x}{x} d x}_{d u} \\
& =x(\ln x)^2-2 \int \ln x d x .
\end{aligned}
$$


So we need $\int \ln x d x$.

Step 3: Recall $\int \ln x d x$
A standard result (which can also be shown by parts) is

$$
\int \ln x d x=x \ln x-x+C
$$


Hence,

$$
-2 \int \ln x d x=-2(x \ln x-x)=-2 x \ln x+2 x
$$

Step 4: Combine everything

$$
\int(\ln x)^2 d x=x(\ln x)^2-2 x \ln x+2 x+C .
$$


We can factor out $x$ if we like:

$$
\int(\ln x)^2 d x=x\left[(\ln x)^2-2 \ln x+2\right]+C
$$

but it's fine to leave it in expanded form.

Final Answer

$$
\int(\ln x)^2 d x=x(\ln x)^2-2 x \ln x+2 x+C.
$$

}\SetValue{Rubric}{%




}\SetValue{Answer}{%

}
\ProcessDATA


 
   
   

   


