\SetValue{SectionAB}{}\SetValue{MainChapter}{}\SetValue{SubChapter}{}\SetValue{Contents}{%

Evaluate the integral.

$$\int\ t\ \sinh \ m t \ d t$$

}\SetValue{Solution}{%

We want to evaluate

$$
\int t \sinh (m t) d t
$$

where $m$ is a constant.

Step 1: Use Integration by Parts
Recall the integration by parts formula:

$$
\int u d v=u v-\int v d u .
$$


Let

$$
u=t, \quad d v=\sinh (m t) d t .
$$


Then

$$
d u=d t, \quad v=\int \sinh (m t) d t .
$$


We know

$$
\int \sinh (m t) d t=\dfrac{1}{m} \cosh (m t)
$$

Hence,

$$
v=\dfrac{1}{m} \cosh (m t)
$$


Step 2: Apply the Formula

$$
\int t \sinh (m t) d t=u v-\int v d u=t \cdot\left(\dfrac{1}{m} \cosh (m t)\right)-\int\left(\dfrac{1}{m} \cosh (m t)\right) d t
$$


Simplify:

$$
=\dfrac{t}{m} \cosh (m t)-\dfrac{1}{m} \int \cosh (m t) d t
$$


Step 3: Integrate $\cosh (m t)$

$$
\int \cosh (m t) d t=\dfrac{1}{m} \sinh (m t)
$$


Thus,

$$
-\dfrac{1}{m} \int \cosh (m t) d t=-\dfrac{1}{m}\left(\dfrac{1}{m} \sinh (m t)\right)=-\dfrac{1}{m^2} \sinh (m t)
$$

Step 4: Combine Everything
Putting it all together:

$$
\int t \sinh (m t) d t=\dfrac{t}{m} \cosh (m t)-\dfrac{1}{m^2} \sinh (m t)+C,
$$

where $C$ is the constant of integration.

Final Answer

$$
\int t \sinh (m t) d t=\dfrac{t}{m} \cosh (m t)-\dfrac{1}{m^2} \sinh (m t)+C \text {. }
$$

}\SetValue{Rubric}{%




}\SetValue{Answer}{%

}
\ProcessDATA


 
   
   

   


