\SetValue{SectionAB}{}\SetValue{MainChapter}{}\SetValue{SubChapter}{}\SetValue{Contents}{%

Evaluate the integral.

$$\int\ z^{3} \ e^z\ d z$$

}\SetValue{Solution}{%

A straightforward way to evaluate

$$
\int z^3 e^z d z
$$

is by using integration by parts repeatedly. Here's a clear step-by-step process.

Integration by Parts Formula
Recall that for functions $u(z)$ and $v(z)$,

$$
\int u d v=u v-\int v d u
$$


Step 1: First Integration by Parts
1. Let

$$
u=z^3, \quad d v=e^z d z
$$

2. Then

$$
d u=3 z^2 d z, \quad v=\int e^z d z=e^z
$$

3. Apply the formula:

$$
\int z^3 e^z d z=z^3 e^z-\int 3 z^2 e^z d z=z^3 e^z-3 \int z^2 e^z d z
$$


Hence we must now handle $\int z^2 e^z d z$.

Step 2: Second Integration by Parts
Consider $\int z^2 e^z d z$ :
1. Let

$$
u=z^2, \quad d v=e^z d z
$$

2. Then

$$
d u=2 z d z, \quad v=e^z
$$

3. Apply the formula:

$$
\int z^2 e^z d z=z^2 e^z-\int 2 z e^z d z=z^2 e^z-2 \int z e^z d z
$$


Now we need $\int z e^z d z$.

Step 3: Third Integration by Parts
Consider $\int z e^z d z$ :
1. Let

$$
u=z, \quad d v=e^z d z
$$

2. Then

$$
d u=d z, \quad v=e^z .
$$

3. Apply the formula:

$$
\int z e^z d z=z e^z-\int e^z d z=z e^z-e^z=e^z(z-1) .
$$


Thus

$$
\int z e^z d z=e^z(z-1)
$$


Step 2 (continued)
Substitute back:

$$
\int z^2 e^z d z=z^2 e^z-2\left[e^z(z-1)\right]=z^2 e^z-2 z e^z+2 e^z=e^z\left(z^2-2 z+2\right)
$$

Step 4: Combine Everything

Recall from Step 1:

$$
\int z^3 e^z d z=z^3 e^z-3 \int z^2 e^z d z=z^3 e^z-3\left[e^z\left(z^2-2 z+2\right)\right]
$$


Distribute the -3 :

$$
=z^3 e^z-3 z^2 e^z+6 z e^z-6 e^z=e^z\left(z^3-3 z^2+6 z-6\right) .
$$


Thus the final result is:

$$
\int z^3 e^z d z=e^z\left(z^3-3 z^2+6 z-6\right)+C
$$

where $C$ is the constant of integration.

}\SetValue{Rubric}{%




}\SetValue{Answer}{%

}
\ProcessDATA


 
   
   

   


