\SetValue{SectionAB}{}\SetValue{MainChapter}{}\SetValue{SubChapter}{}\SetValue{Contents}{%

Evaluate the integral.
   
$$\int\ \dfrac{xe^{2x}}{\left( 1+2x \right)^2 }\ d x$$
   
}\SetValue{Solution}{%

A quick way to see the result is to notice that the expression

$$
\dfrac{x e^{2 x}}{(1+2 x)^2}
$$

resembles the derivative of $\dfrac{e^{2 x}}{1+2 x}$. Indeed, let us compute

$$
\dfrac{d}{d x}\left(\dfrac{e^{2 x}}{1+2 x}\right)
$$

using the quotient rule:

$$
\dfrac{d}{d x}\left(\dfrac{e^{2 x}}{1+2 x}\right)=\dfrac{(1+2 x) \dfrac{d}{d x}\left[e^{2 x}\right]-e^{2 x} \dfrac{d}{d x}[1+2 x]}{(1+2 x)^2}
$$


Since $\dfrac{d}{d x}\left[e^{2 x}\right]=2 e^{2 x}$ and $\dfrac{d}{d x}[1+2 x]=2$, we get

$$
=\dfrac{(1+2 x) \cdot 2 e^{2 x}-e^{2 x} \cdot 2}{(1+2 x)^2}=\dfrac{2 e^{2 x}((1+2 x)-1)}{(1+2 x)^2}=\dfrac{2 e^{2 x}(2 x)}{(1+2 x)^2}=\dfrac{4 x e^{2 x}}{(1+2 x)^2} .
$$


Observe that

$$
\dfrac{x e^{2 x}}{(1+2 x)^2}=\dfrac{1}{4} \dfrac{4 x e^{2 x}}{(1+2 x)^2}=\dfrac{1}{4} \dfrac{d}{d x}\left(\dfrac{e^{2 x}}{1+2 x}\right) .
$$


Hence,

$$
\int \dfrac{x e^{2 x}}{(1+2 x)^2} d x=\int \dfrac{1}{4} \dfrac{d}{d x}\left(\dfrac{e^{2 x}}{1+2 x}\right) d x=\dfrac{1}{4} \dfrac{e^{2 x}}{1+2 x}+C.
$$

Therefore, the integral evaluates to

$$
\int \dfrac{x e^{2 x}}{(1+2 x)^2} d x=\dfrac{e^{2 x}}{4(1+2 x)}+C
$$

}\SetValue{Rubric}{%




}\SetValue{Answer}{%

}
\ProcessDATA


 

