\SetValue{Module}{1}\SetValue{SectionAB}{A}\SetValue{MainChapter}{}\SetValue{SubChapter}{}\SetValue{Contents}{%%
    
Evaluate the integral.

$$\int\ \left( \arcsin \ x \right)^2 \ d x$$

}\SetValue{Concept}{%



}\SetValue{AltText}{%



}\SetValue{Solution}{%

We want to evaluate

$$
I=\int[\arcsin (x)]^2 d x
$$


A natural method is integration by parts, using

$$
\int u d v=u v-\int v d u
$$

1) First integration by parts

Let

$$
u=[\arcsin (x)]^2, \quad d v=d x
$$


Then

$$
d u=2 \arcsin (x) \dfrac{d}{d x}(\arcsin x)=2 \arcsin (x) \dfrac{1}{\sqrt{1-x^2}} d x, \quad v=\int d x=x
$$


Substitute into the integration by parts formula:

$$
I=\int[\arcsin (x)]^2 d x=\underbrace{[\arcsin (x)]^2}_u \underbrace{x}_v-\int \underbrace{x}_v \underbrace{\left(2 \arcsin (x) \dfrac{1}{\sqrt{1-x^2}}\right)}_{d u} d x
$$

Hence,

$$
I=x[\arcsin (x)]^2-2 \int \dfrac{x \arcsin (x)}{\sqrt{1-x^2}} d x
$$


So we have reduced the problem to evaluating

$$
J=\int \dfrac{x \arcsin (x)}{\sqrt{1-x^2}} d x
$$

2) Substitute $x=\sin (t)$ in the remaining integral

Let

$$
x=\sin t \quad \Longrightarrow \quad t=\arcsin (x), \quad d x=\cos t d t, \quad \sqrt{1-x^2}=\sqrt{1-\sin ^2 t}=\cos t \quad\left(\text { assuming } t \in\left[-\dfrac{\pi}{2}, \dfrac{\pi}{2}\right]\right)
$$


Then

$$
J=\int \dfrac{(\sin t)(t)}{\cos t}(\cos t d t)=\int t \sin t d t
$$


Thus we need $\int t \sin t d t$.

2.1) Integrate $\int t \sin t d t$ by parts

Another integration by parts:

- Let $u=t$, so $d u=d t$.

- Let $d v=\sin t d t$, so $v=-\cos t$.

Hence,

$$
\int t \sin t d t=t(-\cos t)-\int(-\cos t) d t=-t \cos t+\int \cos t d t=-t \cos t+\sin t
$$


Therefore,

$$
J=\int t \sin t d t=-t \cos t+\sin t
$$


Returning to $x$-variables: $t=\arcsin (x)$ and $\cos t=\sqrt{1-x^2}, \sin t=x$. So

$$
J=-\arcsin (x) \sqrt{1-x^2}+x
$$

3) Combine results

We found:

$$
I=x[\arcsin (x)]^2-2 \int \dfrac{x \arcsin (x)}{\sqrt{1-x^2}} d x=x[\arcsin (x)]^2-2 J.
$$

But

$$
J=-\arcsin (x) \sqrt{1-x^2}+x
$$


Hence,

$$
-2 J=-2\left(-\arcsin (x) \sqrt{1-x^2}+x\right)=2 \arcsin (x) \sqrt{1-x^2}-2 x
$$


Therefore,

$$
I=x[\arcsin (x)]^2+2 \arcsin (x) \sqrt{1-x^2}-2 x+C
$$

where $C$ is the constant of integration.

Final Answer

$$
\int[\arcsin (x)]^2 d x=x[\arcsin (x)]^2+2 \arcsin (x) \sqrt{1-x^2}-2 x+C
$$

}\SetValue{Rubric}{%Markdown



}\SetValue{Hint}{%
Solution Goes Here
}\SetValue{Answer}{%

}
\ProcessDATA



 
   
   

   


