\SetValue{Module}{1}\SetValue{SectionAB}{A}\SetValue{MainChapter}{}\SetValue{SubChapter}{}\SetValue{Contents}{%%
    
Determine whether the sequence converges or diverges. If it converges, find the limit.

$$\left\{ \frac{e^n+e^{-n}}{e^{2n}-1} \right\}$$

}\SetValue{Concept}{%



}\SetValue{AltText}{%



}\SetValue{Solution}{%

We are given the sequence:

$
a_n = \frac{e^n + e^{-n}}{e^{2n} - 1}
$

We want to determine whether this sequence converges or diverges as $n \to \infty$, and if it converges, find the limit.



 Step 1: Analyze dominant terms as $n \to \infty$

As $n \to \infty$:

- $e^n \to \infty$

- $e^{-n} \to 0$

- $e^{2n} \to \infty$

So the numerator becomes:
$
e^n + e^{-n} \approx e^n
$

And the denominator becomes:
$
e^{2n} - 1 \approx e^{2n}
$

Thus, the sequence behaves like:
$
a_n \approx \frac{e^n}{e^{2n}} = \frac{1}{e^n}
$



 Step 2: Take the limit

$
\lim_{n \to \infty} a_n = \lim_{n \to \infty} \frac{e^n + e^{-n}}{e^{2n} - 1} = \lim_{n \to \infty} \frac{1}{e^n} = 0
$

Final Answer:

The sequence converges, and its limit is:

$
\boxed{0}
$
}\SetValue{Rubric}{%Markdown



}\SetValue{Hint}{%
Solution Goes Here
}\SetValue{Answer}{%

}
\ProcessDATA



