\SetValue{Module}{1}\SetValue{SectionAB}{A}\SetValue{MainChapter}{}\SetValue{SubChapter}{}\SetValue{Contents}{%%
    
Determine whether the sequence converges or diverges. If it converges, find the limit.

$$a_n=\ln\left( 2n^2+1 \right) -\ln\left( n^2+1 \right) $$

}\SetValue{Concept}{%



}\SetValue{AltText}{%



}\SetValue{Solution}{%

We are given the sequence:

$
a_n = \ln(2n^2 + 1) - \ln(n^2 + 1)
$



 Step 1: Use logarithmic properties

Apply the identity:

$
\ln A - \ln B = \ln\left(\frac{A}{B}\right)
$

So we rewrite:

$
a_n = \ln\left( \frac{2n^2 + 1}{n^2 + 1} \right)
$



 Step 2: Simplify the expression

Divide numerator and denominator by $n^2$:

$
\frac{2n^2 + 1}{n^2 + 1} = \frac{2 + \frac{1}{n^2}}{1 + \frac{1}{n^2}} \to \frac{2}{1} = 2 \quad \text{as } n \to \infty
$


 Step 3: Take the limit

$
\lim_{n \to \infty} a_n = \lim_{n \to \infty} \ln\left( \frac{2n^2 + 1}{n^2 + 1} \right) = \ln(2)
$

Final Answer:

The sequence converges, and its limit is:

$
\boxed{\ln 2}
$
}\SetValue{Rubric}{%Markdown



}\SetValue{Hint}{%
Solution Goes Here
}\SetValue{Answer}{%

}
\ProcessDATA



