\SetValue{Module}{1}\SetValue{SectionAB}{A}\SetValue{MainChapter}{}\SetValue{SubChapter}{}\SetValue{Contents}{%%
    
Differentiate.

$y=\sec \theta \tan \theta$

}\SetValue{Concept}{%



}\SetValue{AltText}{%



}\SetValue{Solution}{%

Let
$
y = \sec \theta \,\tan \theta.
$
Apply the product rule $(uv)' = u'v + uv'$. 

Set $u = \sec \theta$ and $v = \tan \theta$. 

Then

$
u' = \dfrac{d}{d\theta} (\sec \theta) = \sec \theta \tan \theta,
\quad
v' = \dfrac{d}{d\theta} (\tan \theta) = \sec^2 \theta.
$

Thus,
$
y' = (\sec \theta \tan \theta)\,(\tan \theta) + (\sec \theta)\,(\sec^2 \theta) 
    = \sec \theta\,\tan^2 \theta + \sec^3 \theta.
$

You can leave the answer in this form or factor further using $\tan^2 \theta = \sec^2 \theta - 1$, giving
$
y' = \sec \theta\,(\tan^2 \theta + \sec^2 \theta) 
    = \sec \theta\bigl((\sec^2 \theta - 1) + \sec^2 \theta\bigr)
    = 2\sec^3 \theta - \sec \theta.
$

Either form is correct.

}\SetValue{Rubric}{%Markdown



}\SetValue{Hint}{%
Solution Goes Here
}\SetValue{Answer}{%

}
\ProcessDATA



