\SetValue{Module}{1}\SetValue{SectionAB}{A}\SetValue{MainChapter}{}\SetValue{SubChapter}{}\SetValue{Contents}{%%
    
Differentiate.

$y=c \cos t+t^2 \sin t$

}\SetValue{Concept}{%



}\SetValue{AltText}{%



}\SetValue{Solution}{%

Given
$
y = c \cos t + t^2 \sin t,
$
where $c$ is a constant, we differentiate term by term:

1. $\dfrac{d}{dt}(c \cos t) = c \cdot (-\sin t) = -c \sin t.$

2. $\dfrac{d}{dt}(t^2 \sin t)$: use the product rule $(uv)' = u'v + uv'$:
   - $u = t^2 \implies u' = 2t.$
   - $v = \sin t \implies v' = \cos t.$
   
Hence,
   $
   \dfrac{d}{dt}(t^2 \sin t) = 2t \sin t + t^2 \cos t.
   $

So,
$
\dfrac{dy}{dt} = -c \sin t + 2t \sin t + t^2 \cos t.
$

}\SetValue{Rubric}{%Markdown



}\SetValue{Hint}{%
Solution Goes Here
}\SetValue{Answer}{%

}
\ProcessDATA



