\SetValue{Module}{1}\SetValue{SectionAB}{A}\SetValue{MainChapter}{}\SetValue{SubChapter}{}\SetValue{Contents}{%%
    
Differentiate.

$f(t)=\dfrac{\cot t}{e^t}$

}\SetValue{Concept}{%



}\SetValue{AltText}{%



}\SetValue{Solution}{%

We have
$
f(t) = \dfrac{\cot t}{e^t}.
$

Use the quotient rule:
$
\biggl(\dfrac{u}{v}\biggr)' 
= \dfrac{u'v - uv'}{v^2},
$

where $u = \cot t$ and $v = e^t$. 

Compute each derivative:

$
u' = \dfrac{d}{dt}(\cot t) = -\csc^2 t,
\quad
v' = \dfrac{d}{dt}(e^t) = e^t.
$

Thus,
$
f'(t) 
= \dfrac{(-\csc^2 t)\,e^t - (\cot t)\,(e^t)}{(e^t)^2}
= \dfrac{e^t\bigl(-\csc^2 t - \cot t\bigr)}{e^{2t}}
= -\,\dfrac{\csc^2 t + \cot t}{e^t}.
$

Hence, in fraction form,
$
\boxed{f'(t) = -\dfrac{\csc^2 t + \cot t}{e^t}.}
$

}\SetValue{Rubric}{%Markdown



}\SetValue{Hint}{%
Solution Goes Here
}\SetValue{Answer}{%

}
\ProcessDATA



