\SetValue{Module}{1}\SetValue{SectionAB}{A}\SetValue{MainChapter}{}\SetValue{SubChapter}{}\SetValue{Contents}{%%
    
Differentiate.

$y=\dfrac{x}{2-\tan x}$

}\SetValue{Concept}{%



}\SetValue{AltText}{%



}\SetValue{Solution}{%

Given
$
y = \dfrac{x}{2 - \tan x},
$
let $u = x$ and $v = 2 - \tan x$. 

Then $u' = 1$ and $v' = -\sec^2 x$. 

By the quotient rule,

$
\biggl(\dfrac{u}{v}\biggr)' 
= \dfrac{u'v - uv'}{v^2},
$

we get
$
y' 
= \dfrac{(1)(2 - \tan x) \;-\; x\bigl(-\sec^2 x\bigr)}{(2 - \tan x)^2}
= \dfrac{2 - \tan x + x\,\sec^2 x}{(2 - \tan x)^2}.
$

}\SetValue{Rubric}{%Markdown



}\SetValue{Hint}{%
Solution Goes Here
}\SetValue{Answer}{%

}
\ProcessDATA



