\SetValue{Module}{1}\SetValue{SectionAB}{A}\SetValue{MainChapter}{}\SetValue{SubChapter}{}\SetValue{Contents}{%%
    
Differentiate.

$y=\sin \theta \cos \theta$

}\SetValue{Concept}{%



}\SetValue{AltText}{%



}\SetValue{Solution}{%

Using the Product Rule or a Trigonometric Identity:

Given
$
y = \sin \theta \,\cos \theta,
$
we can use the product rule $ (uv)' = u'v + uv' $:
$
y' = (\sin \theta)' \cos \theta + \sin \theta \, (\cos \theta)' 
    = (\cos \theta)\cos \theta + (\sin \theta)(- \sin \theta) 
    = \cos^2 \theta - \sin^2 \theta.
$

Recognize that $\cos^2 \theta - \sin^2 \theta = \cos(2\theta)$. 

Thus:

$
\boxed{y' = \cos(2\theta)}.
$

}\SetValue{Rubric}{%Markdown



}\SetValue{Hint}{%
Solution Goes Here
}\SetValue{Answer}{%

}
\ProcessDATA



