\SetValue{Module}{1}\SetValue{SectionAB}{A}\SetValue{MainChapter}{}\SetValue{SubChapter}{}\SetValue{Contents}{%%
    
Differentiate.

$f(\theta)=\dfrac{\sec \theta}{1+\sec \theta}$

}\SetValue{Concept}{%



}\SetValue{AltText}{%



}\SetValue{Solution}{%

Using the Quotient Rule:

We have
$
f(\theta) = \dfrac{\sec \theta}{1 + \sec \theta}.
$
Set $u = \sec \theta$ and $v = 1 + \sec \theta$. 

Then:

$
u' = \sec \theta \tan \theta, 
\quad
v' = \sec \theta \tan \theta.
$

Using the quotient rule,
$
\biggl(\dfrac{u}{v}\biggr)' 
= \dfrac{u'v - uv'}{v^2},
$

we get

$
f'(\theta) 
= \dfrac{\bigl(\sec \theta \tan \theta\bigr)\bigl(1 + \sec \theta\bigr) \;-\; \sec \theta \bigl(\sec \theta \tan \theta\bigr)}{\bigl(1 + \sec \theta\bigr)^2}
= \dfrac{\sec \theta \tan \theta \bigl(1 + \sec \theta\bigr) - \sec^2 \theta \tan \theta}{\bigl(1 + \sec \theta\bigr)^2}.
$

Inside the numerator:
$
\sec \theta \tan \theta \bigl(1 + \sec \theta\bigr) - \sec^2 \theta \tan \theta
= \sec \theta \tan \theta + \sec^2 \theta \tan \theta - \sec^2 \theta \tan \theta
= \sec \theta \tan \theta.
$

Hence,
$
\boxed{f'(\theta) 
= \dfrac{\sec \theta \tan \theta}{\bigl(1 + \sec \theta\bigr)^2}.}
$

}\SetValue{Rubric}{%Markdown



}\SetValue{Hint}{%
Solution Goes Here
}\SetValue{Answer}{%

}
\ProcessDATA



