\SetValue{Module}{1}\SetValue{SectionAB}{A}\SetValue{MainChapter}{}\SetValue{SubChapter}{}\SetValue{Contents}{%%
    
Differentiate.

$y=\dfrac{\cos x}{1-\sin x}$

}\SetValue{Concept}{%



}\SetValue{AltText}{%



}\SetValue{Solution}{%

Using the Quotient Rule:

Given
$
y = \dfrac{\cos x}{1 - \sin x},
$
let $u = \cos x$ and $v = 1 - \sin x$. 

Then

$
u' = -\sin x,
\quad
v' = -\cos x.
$

By the quotient rule,
$
\left(\dfrac{u}{v}\right)' = \dfrac{u'v - uv'}{v^2},
$

we get
$
y' = \dfrac{\bigl(-\sin x\bigr)\bigl(1 - \sin x\bigr) - (\cos x)\bigl(-\cos x\bigr)}{(1 - \sin x)^2}
    = \dfrac{-\sin x(1 - \sin x) + \cos^2 x}{(1 - \sin x)^2}.
$

Simplify the numerator:

$
-\sin x \,(1 - \sin x) + \cos^2 x
= -\sin x + \sin^2 x + \cos^2 x
= -\sin x + 1
= 1 - \sin x.
$

Therefore,

$
y' = \dfrac{1 - \sin x}{(1 - \sin x)^2} = \dfrac{1}{1 - \sin x}.
$

Hence,

$
\boxed{y' = \dfrac{1}{1 - \sin x}.}
$

}\SetValue{Rubric}{%Markdown



}\SetValue{Hint}{%
Solution Goes Here
}\SetValue{Answer}{%

}
\ProcessDATA



