\SetValue{Module}{1}\SetValue{SectionAB}{A}\SetValue{MainChapter}{}\SetValue{SubChapter}{}\SetValue{Contents}{%%
    
Differentiate.

$y=\dfrac{t \sin t}{1+t}$

}\SetValue{Concept}{%



}\SetValue{AltText}{%



}\SetValue{Solution}{%

Using the Quotient Rule:

We have
$
y = \dfrac{t \sin t}{1 + t}.
$
Let $u = t \sin t$ and $v = 1 + t$. 

Then:

$
u' = \dfrac{d}{dt}(t \sin t) = \sin t + t \cos t,\quad
v' = \dfrac{d}{dt}(1 + t) = 1.
$

Using the quotient rule,
$
\left(\dfrac{u}{v}\right)' 
= \dfrac{u'v - uv'}{v^2},
$

we get
$
y' 
= \dfrac{\bigl(\sin t + t \cos t\bigr)\bigl(1 + t\bigr) - \bigl(t \sin t\bigr)\cdot(1)}{(1 + t)^2}.
$

Simplify the numerator:

$
(\sin t + t \cos t)(1 + t) - t \sin t 
= \sin t(1 + t) + t \cos t(1 + t) - t \sin t 
= \sin t + t \sin t + t \cos t + t^2 \cos t - t \sin t.
$

Notice 

$t \sin t - t \sin t$ cancels out:
$
= \sin t + t \cos t + t^2 \cos t.
$

Therefore,
$
\boxed{y' 
= \dfrac{\sin t + t \cos t + t^2 \cos t}{(1 + t)^2}.
}
$

}\SetValue{Rubric}{%Markdown



}\SetValue{Hint}{%
Solution Goes Here
}\SetValue{Answer}{%

}
\ProcessDATA



