\SetValue{Module}{1}\SetValue{SectionAB}{A}\SetValue{MainChapter}{}\SetValue{SubChapter}{}\SetValue{Contents}{%%
    
Differentiate.

$f(x)=x e^x \csc x$

}\SetValue{Concept}{%



}\SetValue{AltText}{%



}\SetValue{Solution}{%

Using the Product Rule with three factors:

We have
$
f(x) = x \, e^x \,\csc x.
$
Think of $f$ as the product $u \cdot v \cdot w$ where
$
u = x,\quad v = e^x,\quad w = \csc x.
$

Then the derivative $f'(x)$ is given by
$
f'(x) 
= u' \, v \, w + u \, v' \, w + u \, v \, w'.
$

Compute each derivative:

1. $u' = \dfrac{d}{dx}(x) = 1.$  

2. $v' = \dfrac{d}{dx}(e^x) = e^x.$  

3. $w' = \dfrac{d}{dx}(\csc x) = -\csc x \cot x.$

Putting it all together:

$
f'(x) 
= (1)\, e^x \,\csc x \;+\; x \, (e^x)\,\csc x \;+\; x \, e^x \,\bigl(-\csc x \cot x\bigr).
$

Simplify:

$
f'(x) 
= e^x \csc x 
  + x e^x \csc x 
  - x e^x \csc x \cot x.
$

You may also factor out the common terms $e^x \csc x$:

$
\boxed{f'(x) 
= e^x \csc x\,\bigl(1 + x - x \cot x\bigr).}
$

}\SetValue{Rubric}{%Markdown



}\SetValue{Hint}{%
Solution Goes Here
}\SetValue{Answer}{%

}
\ProcessDATA



