\SetValue{Module}{1}\SetValue{SectionAB}{A}\SetValue{MainChapter}{}\SetValue{SubChapter}{}\SetValue{Contents}{%%
    
Find the limit.

$\lim _{x \rightarrow \tfrac{\pi}{4}} \dfrac{1-\tan x}{\sin x-\cos x}$

}\SetValue{Concept}{%



}\SetValue{AltText}{%



}\SetValue{Solution}{%

We want to find
$
\lim_{x \to \dfrac{\pi}{4}} \dfrac{1 - \tan x}{\sin x - \cos x}.
$

A direct substitution at $x = \dfrac{\pi}{4}$ yields
$
1 - \tan \bigl(\tfrac{\pi}{4}\bigr) = 1 - 1 = 0, 
\quad
\sin \bigl(\tfrac{\pi}{4}\bigr) - \cos \bigl(\tfrac{\pi}{4}\bigr) 
= \dfrac{\sqrt{2}}{2} - \dfrac{\sqrt{2}}{2} = 0,
$

so the expression is in an indeterminate form $0/0$.

We can apply L’Hôpital’s Rule, which says:

$
\lim_{x \to a} \dfrac{f(x)}{g(x)} 
= \lim_{x \to a} \dfrac{f'(x)}{g'(x)}
\quad
\text{if}~f(a)=g(a)=0.
$

1. Differentiate the numerator $1 - \tan x$:
   $
   \dfrac{d}{dx} \bigl(1 - \tan x\bigr) = 0 - \sec^2 x = -\sec^2 x.
   $

2. Differentiate the denominator $\sin x - \cos x$:
   $
   \dfrac{d}{dx} (\sin x - \cos x) = \cos x + \sin x.
   $

Hence, by L’Hôpital’s Rule,

$
\lim_{x \to \dfrac{\pi}{4}} \dfrac{1 - \tan x}{\sin x - \cos x}
= \lim_{x \to \dfrac{\pi}{4}} \dfrac{-\sec^2 x}{\cos x + \sin x}.
$

Evaluate at $x = \tfrac{\pi}{4}$:

- $\sec \bigl(\tfrac{\pi}{4}\bigr) = \dfrac{1}{\cos(\tfrac{\pi}{4})} = \dfrac{1}{\tfrac{\sqrt{2}}{2}} = \sqrt{2}$, so $\sec^2 (\tfrac{\pi}{4}) = 2$.  

- $\cos\bigl(\tfrac{\pi}{4}\bigr) + \sin\bigl(\tfrac{\pi}{4}\bigr) = \dfrac{\sqrt{2}}{2} + \dfrac{\sqrt{2}}{2} = \sqrt{2}.$

Thus,

$
\dfrac{-\sec^2(\tfrac{\pi}{4})}{\cos(\tfrac{\pi}{4}) + \sin(\tfrac{\pi}{4})}
= \dfrac{-2}{\sqrt{2}}
= -\sqrt{2}.
$

Therefore,

$
\boxed{-\sqrt{2}}.
$

}\SetValue{Rubric}{%Markdown



}\SetValue{Hint}{%
Solution Goes Here
}\SetValue{Answer}{%

}
\ProcessDATA



