\SetValue{Module}{1}\SetValue{SectionAB}{A}\SetValue{MainChapter}{}\SetValue{SubChapter}{}\SetValue{Contents}{%%
    
Find the derivative of the function.

$F(x)=\left(x^4+3 x^2-2\right)^5$

}\SetValue{Concept}{%



}\SetValue{AltText}{%



}\SetValue{Solution}{%

To find the derivative of $F(x) = \bigl(x^4 + 3x^2 - 2\bigr)^5$, use the chain rule:

1. Let $u = x^4 + 3x^2 - 2$. Then $F(x) = (u)^5$.

2. Compute $\dfrac{du}{dx} = 4x^3 + 6x$.

3. Apply the chain rule: 

$$
F'(x) = 5\,\bigl(x^4 + 3x^2 - 2\bigr)^4 \cdot (4x^3 + 6x).
$$

Hence,

$$
\boxed{F'(x) = 5 \left(x^4 + 3x^2 - 2\right)^4 \left(4x^3 + 6x\right).}
$$

}\SetValue{Rubric}{%Markdown



}\SetValue{Hint}{%
Solution Goes Here
}\SetValue{Answer}{%

}
\ProcessDATA



