\SetValue{Module}{1}\SetValue{SectionAB}{A}\SetValue{MainChapter}{}\SetValue{SubChapter}{}\SetValue{Contents}{%%
    
Find the derivative of the function.

$f(z)=\dfrac{1}{z^2+1}$

}\SetValue{Concept}{%



}\SetValue{AltText}{%



}\SetValue{Solution}{%

We can rewrite the function as 

$$
f(z) = (z^2 + 1)^{-1}.
$$

To find $f'(z)$, use the chain rule:

1. Let $u = z^2 + 1$. Then $f(z) = u^{-1}$.

2. Compute $\dfrac{du}{dz} = 2z$.

3. Apply the chain rule:

   $$
   f'(z) = -1 \cdot (z^2 + 1)^{-2} \cdot 2z = -\dfrac{2z}{(z^2 + 1)^2}.
   $$

Hence,

$$
\boxed{f'(z) = -\dfrac{2z}{(z^2 + 1)^2}.}
$$

}\SetValue{Rubric}{%Markdown



}\SetValue{Hint}{%
Solution Goes Here
}\SetValue{Answer}{%

}
\ProcessDATA



