\SetValue{Module}{1}\SetValue{SectionAB}{A}\SetValue{MainChapter}{}\SetValue{SubChapter}{}\SetValue{Contents}{%%
    
Find the derivative of the function.

$y=x e^{-k x}$

}\SetValue{Concept}{%



}\SetValue{AltText}{%



}\SetValue{Solution}{%

To differentiate the function

$$
y = x\, e^{-kx},
$$

use the product rule:

$$
\dfrac{d}{dx}\bigl[x\, e^{-kx}\bigr] 
= \dfrac{d}{dx}[x] \cdot e^{-kx} + x \cdot \dfrac{d}{dx}[e^{-kx}].
$$

1. $\dfrac{d}{dx}[x] = 1.$

2. $\dfrac{d}{dx}[e^{-kx}] = e^{-kx} \cdot \dfrac{d}{dx}(-kx) = -k\,e^{-kx}.$

Substituting, we get:

$$
y' = 1 \cdot e^{-kx} + x \cdot \bigl(-k\,e^{-kx}\bigr) = e^{-kx} - kx\,e^{-kx}.
$$

Factor out $e^{-kx}$ to simplify:

$$
\boxed{y' = e^{-kx}\,\bigl(1 - kx\bigr).}
$$

}\SetValue{Rubric}{%Markdown



}\SetValue{Hint}{%
Solution Goes Here
}\SetValue{Answer}{%

}
\ProcessDATA


