\SetValue{Module}{1}\SetValue{SectionAB}{A}\SetValue{MainChapter}{}\SetValue{SubChapter}{}\SetValue{Contents}{%%
    
Find the derivative of the function.

$y=e^{-2 t} \cos 4 t$

}\SetValue{Concept}{%



}\SetValue{AltText}{%



}\SetValue{Solution}{%

We have 

$$
y(t) = e^{-2t} \cos(4t).
$$

To differentiate this, use the product rule, which states:

$$
\dfrac{d}{dt}\bigl[f(t)g(t)\bigr] = f'(t)g(t) + f(t)g'(t).
$$

1. Let $f(t) = e^{-2t}$. Then $f'(t) = -2 e^{-2t}$.

2. Let $g(t) = \cos(4t)$. Then 
   $$
   g'(t) = -\sin(4t) \cdot 4 = -4 \sin(4t).
   $$

Thus,

$$
y'(t) 
= \bigl(-2 e^{-2t}\bigr) \cos(4t) + e^{-2t}\,\bigl(-4 \sin(4t)\bigr).
$$

Factor out $e^{-2t}$:

$$
y'(t) 
= e^{-2t} \bigl(-2 \cos(4t) - 4 \sin(4t)\bigr).
$$

Hence, the derivative is

$$
\boxed{
y'(t) = e^{-2t} \bigl(-2 \cos(4t) - 4 \sin(4t)\bigr).
}
$$

}\SetValue{Rubric}{%Markdown



}\SetValue{Hint}{%
Solution Goes Here
}\SetValue{Answer}{%

}
\ProcessDATA



