\SetValue{Module}{1}\SetValue{SectionAB}{A}\SetValue{MainChapter}{}\SetValue{SubChapter}{}\SetValue{Contents}{%%
    
Find the derivative of the function.

$h(t)=(t+1)^{\tfrac{2}{3}}\left(2 t^2-1\right)^3$

}\SetValue{Concept}{%



}\SetValue{AltText}{%



}\SetValue{Solution}{%

We want to differentiate

$$
h(t) \;=\; (t+1)^{\tfrac{2}{3}}\,\bigl(2t^2 - 1\bigr)^{3}.
$$

\textbf{1. Identify the factors and use the Product Rule}

Write $h(t) = u(t)\,v(t)$ where

$$
u(t) = (t+1)^{\tfrac{2}{3}}, 
\quad 
v(t) = (2t^2 - 1)^{3}.
$$

Then by the product rule,

$$
h'(t)
= u'(t)\,v(t)\;+\;u(t)\,v'(t).
$$

\textbf{2. Differentiate} $u(t)$

Let $u(t) = (t+1)^{2/3}$.  

Using the chain rule:

1. Inner function: $t+1$, derivative $1$.

2. Outer function: $\bigl(\,\cdot\,\bigr)^{2/3}$, derivative $\tfrac{2}{3}(\,\cdot\,)^{-1/3}$.

Hence,

$$
u'(t) 
= \dfrac{2}{3}\,(t+1)^{-\tfrac{1}{3}}.
$$

\textbf{3. Differentiate} $v(t)$

Let $v(t) = (2t^2 - 1)^3.$  

Again, chain rule:

1. Inner function: $2t^2 -1$, derivative $4t$.

2. Outer function: $\bigl(\,\cdot\,\bigr)^3$, derivative $3(\,\cdot\,)^2$.

Thus,

$$
v'(t) 
= 3\,\bigl(2t^2 -1\bigr)^2 \,\cdot\,4t 
= 12t\,\bigl(2t^2 -1\bigr)^2.
$$

\textbf{4. Combine via the Product Rule}

$$
h'(t)
= u'(t)\,v(t) \;+\; u(t)\,v'(t)
$$
$$
= \Bigl[\dfrac{2}{3}\,(t+1)^{-\tfrac{1}{3}}\Bigr]\!\bigl(2t^2 -1\bigr)^{3}
\;+\;
\bigl(t+1\bigr)^{\tfrac{2}{3}}\!\Bigl[12t\,\bigl(2t^2 -1\bigr)^{2}\Bigr].
$$

In a ``sum form'', you may leave the answer as:

$$
\boxed{
h'(t) 
= \dfrac{2}{3}\,(t+1)^{-\dfrac13}\,\bigl(2t^2 -1\bigr)^{3}
\;+\;
12t\,(t+1)^{\tfrac{2}{3}}\,(2t^2 -1)^{2}.
}
$$

\textbf{5. Optional: A factored version}

If you wish, you can factor out the common terms $(t+1)^{-1/3}\,(2t^2 -1)^2$:

$$
h'(t)
= (t+1)^{-\dfrac13}\,(2t^2 -1)^{2}
\Bigl[
\,\tfrac{2}{3}\,(2t^2 -1)
\;+\;
12t\,\bigl(t+1\bigr)
\Bigr].
$$

Inside the brackets,

$$
\tfrac{2}{3}(2t^2 -1) + 12t(t+1)
= \tfrac{4}{3}t^2 - \tfrac{2}{3} + 12t^2 + 12t
= \tfrac{40}{3}\,t^2 + 12t - \tfrac{2}{3}
= \tfrac{2}{3}\bigl(20\,t^2 +18\,t -1\bigr).
$$

So a completely factored form is

$$
h'(t)
= \dfrac{2}{3}\,(t+1)^{-\tfrac{1}{3}}\,\bigl(2t^2 -1\bigr)^{2}\,\bigl(20t^2 +18t -1\bigr).
$$

Either form is a correct expression for $h'(t)$.

}\SetValue{Rubric}{%Markdown



}\SetValue{Hint}{%
Solution Goes Here
}\SetValue{Answer}{%

}
\ProcessDATA



