\SetValue{Module}{1}\SetValue{SectionAB}{A}\SetValue{MainChapter}{}\SetValue{SubChapter}{}\SetValue{Contents}{%%
    
Find the derivative of the function.

$y=\left(\dfrac{x^2+1}{x^2-1}\right)^3$

}\SetValue{Concept}{%



}\SetValue{AltText}{%



}\SetValue{Solution}{%

We have

$$
y = \left(\dfrac{x^2 + 1}{x^2 - 1}\right)^3.
$$

A convenient way to differentiate is to use the chain rule with an inner function:

\textbf{1. Define the inner function}

   $$
   u(x) \;=\;\dfrac{x^2 + 1}{x^2 - 1}.
   $$

   Then

   $$
   y = \bigl(u(x)\bigr)^3.
   $$

   \textbf{2. Differentiate the outer function} $y = u^3$:

   $$
   \dfrac{dy}{du} = 3u^2.
   $$
   \textbf{3. Differentiate the inner function} $u(x)$ \textbf{using the quotient rule:}

   $$
   u(x) 
   = \dfrac{x^2 + 1}{x^2 - 1}.
   $$

   The quotient rule states

   $$
   \left(\dfrac{f}{g}\right)' 
   = \dfrac{f'g - fg'}{g^2}.
   $$

   Here $f(x) = x^2 + 1$ and $g(x) = x^2 - 1$. 
   
   Then
   $$
   f'(x) = 2x,\quad g'(x) = 2x.
   $$

   So
   $$
   u'(x)
   = \dfrac{(2x)\,(x^2 - 1) \;-\; (x^2 + 1)\,(2x)}{(x^2 - 1)^2}
   = \dfrac{2x\bigl[(x^2 - 1) - (x^2 + 1)\bigr]}{(x^2 - 1)^2}
   = \dfrac{2x\,\bigl(x^2 - 1 - x^2 - 1\bigr)}{(x^2 - 1)^2}
   = \dfrac{2x\,(-2)}{(x^2 - 1)^2}
   = -\dfrac{4x}{(x^2 - 1)^2}.
   $$

   \textbf{4. Apply the chain rule:}

   $$
   y'(x) 
   = \dfrac{dy}{du} \,\cdot\, \dfrac{du}{dx}
   = 3\bigl(u(x)\bigr)^2 \cdot u'(x).
   $$

   Substituting $u(x) = \dfrac{x^2 + 1}{x^2 - 1}$ and $u'(x) = -\tfrac{4x}{(x^2 - 1)^2}$:

   $$
   y'(x) 
   = 3 \Bigl(\dfrac{x^2 + 1}{x^2 - 1}\Bigr)^2
       \times
       \Bigl(-\dfrac{4x}{(x^2 - 1)^2}\Bigr).
   $$

   Combine the factors:

   $$
   y'(x) 
   = -12x\, \dfrac{(x^2 + 1)^2}{(x^2 - 1)^2} \,\dfrac{1}{(x^2 - 1)^2}
   = -12x\, \dfrac{(x^2 + 1)^2}{(x^2 - 1)^4}.
   $$

Either of the following forms is perfectly valid:

- Factorized form using the chain rule directly:
  $$
  \boxed{
    y'(x) 
    = 3\left(\dfrac{x^2 + 1}{x^2 - 1}\right)^{2} 
      \left(-\dfrac{4x}{(x^2 - 1)^{2}}\right),
  }
  $$

  - As a single fraction:
  $$
  \boxed{
    y'(x) 
    = -\,12x\;\dfrac{(x^2 + 1)^2}{(x^2 - 1)^4}.
  }
  $$
  
}\SetValue{Rubric}{%Markdown



}\SetValue{Hint}{%
Solution Goes Here
}\SetValue{Answer}{%

}
\ProcessDATA



