\SetValue{Module}{1}\SetValue{SectionAB}{A}\SetValue{MainChapter}{}\SetValue{SubChapter}{}\SetValue{Contents}{%%
    
Find the derivative of the function.

$f(s)=\sqrt{\dfrac{s^2+1}{s^2+4}}$

}\SetValue{Concept}{%



}\SetValue{AltText}{%



}\SetValue{Solution}{%

We have

$$
f(s) \;=\; \sqrt{\dfrac{s^2 + 1}{s^2 + 4}}
\;=\;
\biggl(\,\dfrac{s^2 + 1}{s^2 + 4}\biggr)^{\tfrac12}.
$$

To differentiate, it is convenient to use the chain rule, regarding the inside as $\displaystyle u(s) = \dfrac{s^2 + 1}{s^2 + 4}$ and the outer function as $(\,\cdot\,)^{1/2}$.

\textbf{1. Differentiate the outer function}

If $f(s) = \bigl(u(s)\bigr)^{1/2}$, then by the chain rule,

$$
f'(s) 
= \tfrac12\,\bigl(u(s)\bigr)^{-\tfrac12}\;\cdot\;u'(s)
\;=\;
\dfrac{1}{2\sqrt{u(s)}}\,u'(s).
$$

Here, $u(s) = \tfrac{s^2 + 1}{s^2 + 4}$.

\textbf{2. Differentiate the inner function} $u(s)$

Use the quotient rule for

$$
u(s) \;=\; \dfrac{s^2 + 1}{s^2 + 4}.
$$

Let $f(s) = s^2 + 1$ and $g(s) = s^2 + 4$. Then:

- $f'(s) = 2s,\quad g'(s) = 2s.$

- The quotient rule: 
  $$
  \Bigl(\dfrac{f}{g}\Bigr)' 
  = \dfrac{f'\,g \;-\; f\,g'}{g^2}.
  $$

Hence,

$$
u'(s)
= \dfrac{\bigl(2s\bigr)\,(s^2 + 4)\;-\;\bigl(s^2 + 1\bigr)\,(2s)}{(s^2 + 4)^2}
= \dfrac{2s\,[(s^2 + 4) - (s^2 + 1)]}{(s^2 + 4)^2}
= \dfrac{2s\,(3)}{(s^2 + 4)^2}
= \dfrac{6s}{(s^2 + 4)^2}.
$$

\textbf{3. Combine via the chain rule}

Putting it all together:

$$
f'(s) 
= \dfrac{1}{2\sqrt{\tfrac{s^2 + 1}{s^2 + 4}}}
\;\times\;
\dfrac{6s}{(s^2 + 4)^2}.
$$

We can simplify the factor $\dfrac{1}{\sqrt{\tfrac{s^2 + 1}{s^2 + 4}}}$.  Recall

$$
\sqrt{\dfrac{s^2+1}{s^2+4}}
\;=\;
\dfrac{\sqrt{s^2+1}}{\sqrt{s^2+4}}
\quad\Longrightarrow\quad
\dfrac{1}{\sqrt{\dfrac{s^2+1}{s^2+4}}}
\;=\;
\dfrac{\sqrt{s^2+4}}{\sqrt{s^2+1}}.
$$

Hence,

$$
f'(s)
= \dfrac{6s}{2}\,\cdot\,\dfrac{\sqrt{s^2+4}}{\sqrt{s^2+1}}\;\cdot\;\dfrac{1}{(s^2+4)^2}
\;=\;
3s\,\dfrac{\sqrt{s^2+4}}{(s^2+4)^2\,\sqrt{s^2+1}}.
$$

Notice that $\sqrt{s^2+4}$ in the numerator will partially cancel with $(s^2+4)^2$ in the denominator:

$$
\dfrac{\sqrt{s^2+4}}{(s^2+4)^2}
\;=\;
\dfrac{1}{(s^2+4)^{\tfrac{3}{2}}}.
$$

Therefore,

$$
f'(s)
= 3s\,\dfrac{1}{(s^2+4)^{\tfrac{3}{2}}}\,\dfrac{1}{\sqrt{s^2+1}}
\;=\;
\boxed{
\dfrac{3s}{(s^2+4)^{\tfrac{3}{2}}\,\sqrt{s^2+1}}
}.
$$

Either of the following is perfectly acceptable as a final answer:

1. Partially factored:  
   $\displaystyle
   f'(s)
   = \dfrac{1}{2\sqrt{\tfrac{s^2 + 1}{s^2 + 4}}}\,\cdot \dfrac{6s}{(s^2+4)^2}
   $

2. Fully simplified:  
   $\displaystyle
   \boxed{
   f'(s) = \dfrac{3s}{(s^2+4)^{3/2}\,\sqrt{s^2+1}}
   }.$
   
}\SetValue{Rubric}{%Markdown



}\SetValue{Hint}{%
Solution Goes Here
}\SetValue{Answer}{%

}
\ProcessDATA



