\SetValue{Module}{1}\SetValue{SectionAB}{A}\SetValue{MainChapter}{}\SetValue{SubChapter}{}\SetValue{Contents}{%%
    
Find the derivative of the function.

$y=\sqrt{1+2 e^{3 x}}$

}\SetValue{Concept}{%



}\SetValue{AltText}{%



}\SetValue{Solution}{%

To differentiate 

$$
y = \sqrt{1 + 2 e^{3x}} = \bigl(1 + 2 e^{3x}\bigr)^{\tfrac{1}{2}},
$$

use the chain rule:

1. Let $u(x) = 1 + 2 e^{3x}$.

2. Then $y = \bigl(u(x)\bigr)^{1/2}$.

Step A: Differentiate the outer function $(u)^{1/2}$:

$$
\dfrac{d}{du} \bigl(u^{1/2}\bigr)
= \tfrac12\,u^{-1/2}.
$$

Step B: Differentiate the inner function $u(x) = 1 + 2 e^{3x}$:

$$
u'(x) = 2\,\dfrac{d}{dx}\bigl(e^{3x}\bigr)
= 2\cdot 3\,e^{3x}
= 6\,e^{3x}.
$$

Step C: Combine via the chain rule:

$$
y'(x)
= \dfrac12\,(1 + 2 e^{3x})^{-\tfrac12} \;\times\; \bigl[\,6\,e^{3x}\bigr]
= \dfrac{6\,e^{3x}}{2\,\sqrt{1 + 2 e^{3x}}}
= \dfrac{3\,e^{3x}}{\sqrt{1 + 2 e^{3x}}}.
$$

Hence, the derivative is

$$
\boxed{
\dfrac{dy}{dx} = \dfrac{3 e^{3x}}{\sqrt{1 + 2 e^{3x}}}.
}
$$

}\SetValue{Rubric}{%Markdown



}\SetValue{Hint}{%
Solution Goes Here
}\SetValue{Answer}{%

}
\ProcessDATA



