\SetValue{Module}{1}\SetValue{SectionAB}{A}\SetValue{MainChapter}{}\SetValue{SubChapter}{}\SetValue{Contents}{%%
    
Find the derivative of the function.

$y=5^{-\tfrac{1}{x}}$

}\SetValue{Concept}{%



}\SetValue{AltText}{%



}\SetValue{Solution}{%

We want to differentiate

$$
y = 5^{-\tfrac{1}{x}}.
$$

A straightforward way is to rewrite this in exponential form and apply the chain rule:

1. Rewrite $5^{-\dfrac{1}{x}}$ as an exponential with base $e$:

   $$
   y 
   = 5^{-\dfrac{1}{x}}
   = e^{\ln\!\bigl(5^{-\dfrac{1}{x}}\bigr)}
   = e^{-\dfrac{1}{x} \,\ln(5)}.
   $$

   Define
   $$
   u(x) = -\tfrac{1}{x}.
   $$
   Then
   $$
   y = e^{\,u(x)\,\ln(5)}.
   $$

2. Differentiate $y$ via the chain rule:

   $$
   \dfrac{dy}{dx}
   = \dfrac{d}{dx}\bigl[e^{\,u(x)\,\ln(5)}\bigr]
   = e^{\,u(x)\,\ln(5)} \;\cdot\; \dfrac{d}{dx}\bigl(u(x)\,\ln(5)\bigr).
   $$

   Because $\ln(5)$ is constant, we get

   $$
   \dfrac{d}{dx}\bigl(u(x)\,\ln(5)\bigr)
   = \ln(5)\,\dfrac{du}{dx}.
   $$

3. Compute $\dfrac{du}{dx}$ where $u(x) = -\tfrac{1}{x}$:

   $$
   u(x) = -x^{-1}.
   $$

   Its derivative is

   $$
   u'(x)
   = -\bigl(-x^{-2}\bigr)
   = \dfrac{1}{x^2}.
   $$

4. Combine everything:

   $$
   \dfrac{dy}{dx}
   = e^{\,u(x)\,\ln(5)} \;\cdot\;\ln(5)\;\cdot\;\dfrac{1}{x^2}
   = 5^{-\tfrac{1}{x}}\;\ln(5)\;\dfrac{1}{x^2}.
   $$

Thus, the derivative is

$$
\boxed{
\dfrac{dy}{dx}
= \dfrac{\ln(5)\,5^{-\dfrac{1}{x}}}{x^2}.
}
$$

}\SetValue{Rubric}{%Markdown



}\SetValue{Hint}{%
Solution Goes Here
}\SetValue{Answer}{%

}
\ProcessDATA



