\SetValue{Module}{1}\SetValue{SectionAB}{A}\SetValue{MainChapter}{}\SetValue{SubChapter}{}\SetValue{Contents}{%%
    
Find the derivative of the function.

$G(y)=\dfrac{(y-1)^4}{\left(y^2+2 y\right)^5}$

}\SetValue{Concept}{%



}\SetValue{AltText}{%



}\SetValue{Solution}{%

We have

$$
G(y) = \dfrac{(y-1)^4}{\bigl(y^2 + 2y\bigr)^5}.
$$

It can be helpful to treat this as a product:

$$
G(y) \;=\; (y-1)^4\,\bigl(y^2 + 2y\bigr)^{-5}.
$$

Let 

$$
u(y) \;=\; (y-1)^4
\quad\text{and}\quad 
v(y) \;=\; (y^2 + 2y)^{-5}.
$$

Then

$$
G(y) \;=\; u(y)\,v(y).
$$

\textbf{Step 1. Differentiate} $u(y)$

$$
u(y) = (y-1)^4 
\quad\Longrightarrow\quad
u'(y) = 4\,(y-1)^3.
$$

\textbf{Step 2. Differentiate} $v(y)$

$$
v(y) = (y^2 + 2y)^{-5}.
$$

We first note that if $w(y) = y^2 + 2y$, then $w'(y) = 2y + 2$.  
Using the chain rule:

$$
v'(y) 
= -5\,(y^2 + 2y)^{-6}\,\cdot (2y + 2).
$$

\textbf{Step 3. Apply the product rule}

$$
G'(y) 
= u'(y)\,v(y) \;+\; u(y)\,v'(y)
$$
$$
= \Bigl[\,4\,(y-1)^3\Bigr]\!\Bigl[(y^2 + 2y)^{-5}\Bigr]
\;+\;
\Bigl[(y-1)^4\Bigr]\!\Bigl[-5\,(y^2 + 2y)^{-6}\,(2y + 2)\Bigr].
$$

In a ``sum of terms'' form, this is perfectly correct:

$$
G'(y)
= 4(y-1)^3\,(y^2 + 2y)^{-5} 
\;-\; 5\,(y-1)^4\,(2y+2)\,(y^2 + 2y)^{-6}.
$$

\textbf{Optional: Factor out common terms}

Sometimes, it helps to factor out the greatest common factors. Notice that:

- The first term has factors $(y-1)^3$ and $(y^2+2y)^{-5}$.

- The second term has $(y-1)^4$ and $(y^2+2y)^{-6}$.

A common factor is $(y-1)^3 (y^2 + 2y)^{-6}$. Let's factor that out:

$$
G'(y)
= (y-1)^3\,(y^2 + 2y)^{-6}\,\Bigl[\;4\,(y^2+2y)\;-\;5\,(y-1)\,(2y+2)\Bigr].
$$

Inside the bracket:

1. The first piece is $4(y^2+2y)$.

2. The second piece is $\,5\,(y-1)(2y+2)$.

So

$$
[\,\dots\,]
= 4(y^2+2y) \;-\; 5(y-1)(2y+2).
$$

We can expand and simplify further if desired:

- $4(y^2+2y) = 4y^2 + 8y$.

- $(y-1)(2y+2) = 2y(y-1) + 2(y-1) = 2y^2 - 2y + 2y - 2 = 2y^2 - 2.$  
  (Another direct expansion: $(y-1)(2y+2) = 2y^2 + 2y -2y -2 = 2y^2 -2.$)

Hence:

$$
5\,(y-1)(2y+2) 
= 5\,[2y^2 - 2] 
= 10y^2 - 10.
$$

Thus,

$$
[\,\dots\,]
= (4y^2 + 8y) \;-\; (10y^2 - 10)
= 4y^2 + 8y - 10y^2 + 10
= -6y^2 + 8y + 10.
$$

Putting it all together in factored form:

$$
G'(y)
= (y-1)^3\,(y^2 + 2y)^{-6}\,\bigl[-6y^2 + 8y + 10\bigr].
$$

Either the expanded form or the factored form is valid:

$$
\boxed{
G'(y) 
= 4(y-1)^3\,(y^2 + 2y)^{-5}
\;-\;
5\,(y-1)^4\,(2y+2)\,(y^2 + 2y)^{-6},
}
$$

or (factored version)

$$
\boxed{
G'(y)
= (y-1)^3\,(y^2 + 2y)^{-6}\,\bigl[-6y^2 + 8y + 10\bigr].
}
$$

}\SetValue{Rubric}{%Markdown



}\SetValue{Hint}{%
Solution Goes Here
}\SetValue{Answer}{%

}
\ProcessDATA



