\SetValue{Module}{1}\SetValue{SectionAB}{A}\SetValue{MainChapter}{}\SetValue{SubChapter}{}\SetValue{Contents}{%%
    
Find the derivative of the function.

$y=\dfrac{r}{\sqrt{r^2+1}}$

}\SetValue{Concept}{%



}\SetValue{AltText}{%



}\SetValue{Solution}{%

We want to find the derivative of

$$
y(r) = \dfrac{r}{\sqrt{r^2 + 1}}.
$$

A straightforward way is to view $y$ as a product of two functions:

$$
y(r) = r \cdot (r^2 + 1)^{-\tfrac12}.
$$

Let 

$$
u(r) = r, 
\quad
v(r) = (r^2 + 1)^{-\tfrac12}.
$$

Then by the product rule,

$$
y'(r) 
= u'(r)\,v(r) \;+\; u(r)\,v'(r).
$$

\textbf{Step 1: Differentiate} $u(r)$

$$
u(r) = r
\quad\Longrightarrow\quad
u'(r) = 1.
$$

\textbf{Step 2: Differentiate} $v(r)$

$$
v(r) = (r^2 + 1)^{-\tfrac12}.
$$

Use the chain rule:

1. Inner function $g(r) = r^2 + 1$ has derivative $g'(r) = 2r.$

2. Outer function $(\cdot)^{-\tfrac12}$ has derivative $-\tfrac12(\cdot)^{-\tfrac32}.$

Hence,

$$
v'(r) 
= -\tfrac12\,(r^2 + 1)^{-\tfrac32} \;\cdot\;2r 
= -r\,(r^2 + 1)^{-\tfrac32}.
$$

\textbf{Step 3: Combine via the product rule}

$$
y'(r)
= \bigl[\,1\bigr]\!\bigl[(r^2 + 1)^{-\tfrac12}\bigr]
\;+\;
\bigl[\,r\bigr]\!\bigl[-r\,(r^2 + 1)^{-\tfrac32}\bigr].
$$

So,

$$
y'(r)
= (r^2 + 1)^{-\tfrac12}
\;-\;
r^2\,(r^2 + 1)^{-\tfrac32}.
$$

Now factor out $(r^2 + 1)^{-\tfrac32}$:

$$
(r^2 + 1)^{-\tfrac12} 
= (r^2 + 1)^{-\tfrac32} \,(r^2 + 1),
$$

so

$$
y'(r)
= (r^2 + 1)\,(r^2 + 1)^{-\tfrac32}
\;-\;
r^2\,(r^2 + 1)^{-\tfrac32}
= \bigl[(r^2 + 1) - r^2\bigr]\,(r^2 + 1)^{-\tfrac32}
= (1)\,(r^2 + 1)^{-\tfrac32}.
$$

Hence,

$$
\boxed{
y'(r) 
= \dfrac{1}{\bigl(r^2 + 1\bigr)^{\tfrac32}}.
}
$$

}\SetValue{Rubric}{%Markdown



}\SetValue{Hint}{%
Solution Goes Here
}\SetValue{Answer}{%

}
\ProcessDATA



