\SetValue{Module}{1}\SetValue{SectionAB}{A}\SetValue{MainChapter}{}\SetValue{SubChapter}{}\SetValue{Contents}{%%
    
Find the derivative of the function.

$y=\dfrac{e^u-e^{-u}}{e^u+e^{-u}}$

}\SetValue{Concept}{%



}\SetValue{AltText}{%



}\SetValue{Solution}{%

First, note that the given function

$$
y(u) = \dfrac{e^u - e^{-u}}{e^u + e^{-u}}
$$

is the standard definition of the hyperbolic tangent:

$$
y(u) = \tanh(u).
$$

A well‚Äêknown fact about $\tanh(u)$ is that

$$
\dfrac{d}{du}\bigl[\tanh(u)\bigr]
=
\operatorname{sech}^2(u)
=
1 - \tanh^2(u).
$$

Hence, recognizing the function as $\tanh(u)$ immediately gives

$$
\boxed{ y'(u) = 1 - y(u)^2 = \operatorname{sech}^2(u). }
$$

\textbf{Derivation via the Quotient Rule}

If you prefer to differentiate $\displaystyle y(u) = \dfrac{e^u - e^{-u}}{e^u + e^{-u}}$ directly, use the quotient rule.  Let

$$
\text{Numerator: } T(u) = e^u - e^{-u}, 
\quad
\text{Denominator: } B(u) = e^u + e^{-u}.
$$

Then

$$
T'(u) 
= \dfrac{d}{du}\bigl(e^u - e^{-u}\bigr) 
= e^u -\bigl(-e^{-u}\bigr) 
= e^u + e^{-u},
$$
$$
B'(u)
= \dfrac{d}{du}\bigl(e^u + e^{-u}\bigr)
= e^u - e^{-u}.
$$

By the quotient rule,

$$
y'(u)
= \dfrac{T'(u)\,B(u) - T(u)\,B'(u)}{\bigl[B(u)\bigr]^2}
= \dfrac{(e^u + e^{-u})(e^u + e^{-u}) - (e^u - e^{-u})(e^u - e^{-u})}
       {\bigl(e^u + e^{-u}\bigr)^2}.
$$

Observe the numerator:

$$
(e^u + e^{-u})^2 
= e^{2u} + 2 + e^{-2u},
$$
$$
(e^u - e^{-u})^2 
= e^{2u} - 2 + e^{-2u}.
$$

Their difference is 

$$
\bigl(e^{2u} + 2 + e^{-2u}\bigr)
-
\bigl(e^{2u} - 2 + e^{-2u}\bigr)
= 4.
$$

Hence the numerator is $4$, and so

$$
y'(u)
= \dfrac{4}{\bigl(e^u + e^{-u}\bigr)^2}.
$$

One can also verify that 

$\operatorname{sech}^2(u) = \dfrac{4}{(e^u + e^{-u})^2}$, matching the known identity for $\tanh(u)$.

\textbf{Summary}

1. Using the hyperbolic identity:  
   $$
   y(u) = \tanh(u) 
   \quad\Longrightarrow\quad
   y'(u) = \operatorname{sech}^2(u) = 1 - \tanh^2(u) = 1 - y^2.
   $$

2. Using the quotient rule:  
   $$
    \boxed{ 
   y'(u) 
   = \dfrac{4}{\bigl(e^u + e^{-u}\bigr)^2}.
   }$$

Both expressions are correct and equivalent. The most concise answer is:

$$
\dfrac{dy}{du} = 1 - \bigl(\tanh(u)\bigr)^2 = \operatorname{sech}^2(u).
$$

}\SetValue{Rubric}{%Markdown



}\SetValue{Hint}{%
Solution Goes Here
}\SetValue{Answer}{%

}
\ProcessDATA


