\SetValue{Module}{1}\SetValue{SectionAB}{A}\SetValue{MainChapter}{}\SetValue{SubChapter}{}\SetValue{Contents}{%%
    
Find the derivative of the function.

$F(t)=e^{t \sin 2 t}$

}\SetValue{Concept}{%



}\SetValue{AltText}{%



}\SetValue{Solution}{%

We have

$$
F(t) = e^{t \sin(2t)}.
$$

To differentiate this, use the chain rule. Let

$$
g(t) = t \sin(2t).
$$

Then

$$
F(t) = e^{g(t)}.
$$

By the chain rule,

$$
F'(t)
= e^{g(t)} \, g'(t).
$$
Hence we need $g'(t)$.

\textbf{Differentiating} $g(t)$

$$
g(t) = t \sin(2t).
$$

Apply the product rule:

$$
g'(t)
= \bigl(\sin(2t)\bigr) \cdot \dfrac{d}{dt}[t]
+ t \cdot \dfrac{d}{dt}\bigl[\sin(2t)\bigr].
$$

1. $\dfrac{d}{dt}[t] = 1.$

2. $\dfrac{d}{dt}[\sin(2t)] = \cos(2t)\cdot 2 = 2\cos(2t).$

So
$$
g'(t) = \sin(2t) + 2t \cos(2t).
$$

\textbf{Combine via the chain rule}

$$
F'(t) 
= e^{t \sin(2t)} \; \bigl[\sin(2t) + 2t \cos(2t)\bigr].
$$

Thus, the derivative is:

$$
\boxed{
F'(t) = e^{t \sin(2t)} \,\bigl(\,\sin(2t) + 2t\,\cos(2t)\bigr).
}
$$

}\SetValue{Rubric}{%Markdown



}\SetValue{Hint}{%
Solution Goes Here
}\SetValue{Answer}{%

}
\ProcessDATA



