\SetValue{Module}{1}\SetValue{SectionAB}{A}\SetValue{MainChapter}{}\SetValue{SubChapter}{}\SetValue{Contents}{%%
    
Find the derivative of the function.

$F(v)=\left(\dfrac{v}{v^3+1}\right)^6$

}\SetValue{Concept}{%



}\SetValue{AltText}{%



}\SetValue{Solution}{%

We want the derivative of

$$
F(v) \;=\; \Bigl(\tfrac{v}{v^3 + 1}\Bigr)^{6}.
$$

\textbf{1. Set up for the chain rule}

Let 
$$
u(v) \;=\; \dfrac{v}{v^3 + 1}.
$$

Then
$$
F(v) \;=\; \bigl(u(v)\bigr)^{6}.
$$

By the chain rule,

$$
F'(v) 
= 6\,\bigl(u(v)\bigr)^{5}\;u'(v).
$$

Hence we must find $u'(v)$.

\textbf{2. Differentiate} $u(v) = \dfrac{v}{v^3 + 1}$

Use the quotient rule. Let the numerator be $f(v) = v$ and denominator be $g(v) = v^3 + 1$. Then

$$
f'(v) = 1,
\quad
g'(v) = 3v^2.
$$

By the quotient rule,

$$
u'(v)
= \dfrac{f'(v)\,g(v) \;-\; f(v)\,g'(v)}{\bigl(g(v)\bigr)^2}
= \dfrac{(1)\,(v^3 + 1) - v\,(3v^2)}{(v^3 + 1)^2}
= \dfrac{v^3 + 1 - 3v^3}{(v^3 + 1)^2}
= \dfrac{1 - 2v^3}{(v^3 + 1)^2}.
$$

\textbf{3. Combine via the chain rule}

Substitute back into $F'(v) = 6\,(u(v))^5\,u'(v)$:

$$
F'(v)
= 6 \,\Bigl(\dfrac{v}{v^3+1}\Bigr)^{5}\,\dfrac{1 - 2v^3}{(v^3 + 1)^2}.
$$

You can leave it in this form or simplify further.  Notice

$$
\Bigl(\dfrac{v}{v^3+1}\Bigr)^{5} 
= \dfrac{v^5}{(v^3+1)^5}.
$$

Thus,

$$
F'(v)
= 6 \cdot \dfrac{v^5}{(v^3+1)^5} \; \cdot \; \dfrac{1 - 2v^3}{(v^3+1)^2}
= \dfrac{6\,v^5\,\bigl(1 - 2v^3\bigr)}{(v^3+1)^{7}}.
$$

Either form is correct. A fully simplified form is:

$$
\boxed{
F'(v)
= \dfrac{6\,v^5\,\bigl(1 - 2v^3\bigr)}{\bigl(v^3 + 1\bigr)^{7}}.
}
$$

}\SetValue{Rubric}{%Markdown



}\SetValue{Hint}{%
Solution Goes Here
}\SetValue{Answer}{%

}
\ProcessDATA



