\SetValue{Module}{1}\SetValue{SectionAB}{A}\SetValue{MainChapter}{}\SetValue{SubChapter}{}\SetValue{Contents}{%%
    
Find the derivative of the function.

$y=2^{\sin \pi x}$

}\SetValue{Concept}{%



}\SetValue{AltText}{%



}\SetValue{Solution}{%

We want to differentiate

$$
y(x) \;=\; 2^{\sin(\pi x)}.
$$

A convenient approach is to rewrite $2^{\sin(\pi x)}$ in terms of the natural exponential:

$$
2^{\sin(\pi x)}
= e^{\ln(2)\,\sin(\pi x)}.
$$

\textbf{Step 1: Set up the chain rule}

Let 
$$
g(x) = \ln(2)\,\sin(\pi x).
$$

Then 
$$
y(x) = e^{g(x)}.
$$

By the chain rule,

$$
y'(x) 
= e^{g(x)} \cdot g'(x).
$$

\textbf{Step 2: Differentiate} $g(x)$

$$
g(x) = \ln(2)\,\sin(\pi x).
$$

We can treat $\ln(2)$ as a constant. Then

$$
g'(x)
= \ln(2)\,\dfrac{d}{dx}[\sin(\pi x)]
= \ln(2)\,\bigl[\cos(\pi x)\cdot \pi\bigr]
= \pi\,\ln(2)\,\cos(\pi x).
$$

\textbf{Step 3: Combine}

$$
y'(x)
= e^{g(x)}\cdot \bigl[\pi\,\ln(2)\,\cos(\pi x)\bigr]
= \pi\,\ln(2)\,\cos(\pi x)\;e^{\ln(2)\,\sin(\pi x)}.
$$

Rewriting $e^{\ln(2)\,\sin(\pi x)}$ back as $2^{\sin(\pi x)}$, we get

$$
\boxed{
y'(x) 
= \pi\,\ln(2)\,\cos(\pi x)\;2^{\sin(\pi x)}.
}
$$
}\SetValue{Rubric}{%Markdown



}\SetValue{Hint}{%
Solution Goes Here
}\SetValue{Answer}{%

}
\ProcessDATA



