\SetValue{Module}{1}\SetValue{SectionAB}{A}\SetValue{MainChapter}{}\SetValue{SubChapter}{}\SetValue{Contents}{%%
    
Find the derivative of the function.

$y=x^2 e^{-\tfrac{1}{x}}$

}\SetValue{Concept}{%



}\SetValue{AltText}{%



}\SetValue{Solution}{%

We want to differentiate

$$
y(x) \;=\; x^2 \, e^{-\tfrac{1}{x}}.
$$

\textbf{Step 1: Use the Product Rule}

Let

$$
u(x) = x^2
\quad\text{and}\quad
v(x) = e^{-\tfrac{1}{x}}.
$$

Then

$$
y(x) = u(x) \, v(x).
$$

By the product rule:

$$
y'(x) 
= u'(x)\,v(x) \;+\; u(x)\,v'(x).
$$

\textbf{1a. Differentiate} $u(x) = x^2$

$$
u'(x) = 2x.
$$

\textbf{1b. Differentiate} $v(x) = e^{-\tfrac{1}{x}}$

Use the chain rule: let $w(x) = -\tfrac{1}{x} = -x^{-1}$. Then

- $w'(x) = - \bigl(-1 x^{-2}\bigr) = +x^{-2} = \tfrac{1}{x^2}.$ 

- Thus
  $$
  v'(x) = \dfrac{d}{dx}\bigl[e^{w(x)}\bigr]
  = e^{w(x)} \cdot w'(x)
  = e^{-\tfrac{1}{x}}\cdot \dfrac{1}{x^2}.
  $$

Hence

$$
v'(x) 
= \dfrac{e^{-\tfrac{1}{x}}}{x^2}.
$$

\textbf{Step 2: Combine}

Substitute into the product rule:

$$
y'(x)
= u'(x)\,v(x) + u(x)\,v'(x)
= \bigl[2x\bigr]\bigl[e^{-\tfrac{1}{x}}\bigr] \;+\; \bigl[x^2\bigr]\Bigl[\dfrac{e^{-\tfrac{1}{x}}}{x^2}\Bigr].
$$

Simplify term by term:

1. $2x \, e^{-\tfrac{1}{x}}$ stays as is.

2. $x^2 \times \dfrac{1}{x^2} = 1$, so the second term is simply $e^{-\tfrac{1}{x}}$.

Therefore,

$$
y'(x)
= 2x\,e^{-\tfrac{1}{x}} + e^{-\tfrac{1}{x}}
= e^{-\tfrac{1}{x}} \bigl(2x + 1\bigr).
$$

So the final derivative is:

$$
\boxed{
y'(x) = e^{-\tfrac{1}{x}}\,\bigl(2x + 1\bigr).
}
$$

}\SetValue{Rubric}{%Markdown



}\SetValue{Hint}{%
Solution Goes Here
}\SetValue{Answer}{%

}
\ProcessDATA



