\SetValue{Module}{1}\SetValue{SectionAB}{A}\SetValue{MainChapter}{}\SetValue{SubChapter}{}\SetValue{Contents}{%%
    
Find the derivative of the function.

$y=\cos \left(\dfrac{1-e^{2 x}}{1+e^{2 x}}\right)$

}\SetValue{Concept}{%



}\SetValue{AltText}{%



}\SetValue{Solution}{%

We want to differentiate

$$
y(x) \;=\; \cos\!\Bigl(\dfrac{1 - e^{2x}}{1 + e^{2x}}\Bigr).
$$

\textbf{1. Use the chain rule}

Let 
$$
u(x) \;=\; \dfrac{1 - e^{2x}}{1 + e^{2x}}.
$$
Then $y = \cos(u)$.  By the chain rule,

$$
y'(x) 
= -\sin\bigl(u(x)\bigr)\;u'(x).
$$

Hence we need to compute $u'(x)$.

\textbf{2. Differentiate} $u(x) = \dfrac{1 - e^{2x}}{1 + e^{2x}}$

Use the quotient rule.  Set

$$
\text{Numerator: } f(x) = 1 - e^{2x}, 
\quad
\text{Denominator: } g(x) = 1 + e^{2x}.
$$

Then

$$
f'(x) = -\,2\,e^{2x}, 
\qquad
g'(x) = 2\,e^{2x}.
$$

By the quotient rule,

$$
u'(x)
= \dfrac{\,f'(x)\,g(x)\;-\;f(x)\,g'(x)\,}{\bigl[g(x)\bigr]^2}
= \dfrac{(-2 e^{2x})(1 + e^{2x}) \;-\; (1 - e^{2x})(2 e^{2x})}
       {\bigl(1 + e^{2x}\bigr)^2}.
$$

Compute the numerator carefully:

1. $f'(x)\,g(x) = (-2 e^{2x})(1 + e^{2x}) = -2 e^{2x} - 2 e^{4x}.$

2. $f(x)\,g'(x) = (1 - e^{2x})(2 e^{2x}) = 2 e^{2x} - 2 e^{4x}.$

So the difference is

$$
\bigl[-2 e^{2x} \;-\; 2 e^{4x}\bigr] 
\;-\;
\bigl[2 e^{2x} \;-\; 2 e^{4x}\bigr]
= -2 e^{2x} - 2 e^{4x} - 2 e^{2x} + 2 e^{4x}
= -4 e^{2x}.
$$

Thus,

$$
u'(x)
= \dfrac{-4 e^{2x}}{\bigl(1 + e^{2x}\bigr)^2}.
$$

\textbf{3. Combine via the chain rule}

$$
y'(x)
= -\sin\Bigl(\dfrac{1 - e^{2x}}{1 + e^{2x}}\Bigr) 
\;\times\;
\Bigl[\,-\dfrac{4 e^{2x}}{(1 + e^{2x})^2}\Bigr].
$$

The two negatives multiply to give a positive:

$$
y'(x)
= \dfrac{4\,e^{2x}}{\bigl(1 + e^{2x}\bigr)^2}
\,\sin\!\Bigl(\tfrac{1 - e^{2x}}{1 + e^{2x}}\Bigr).
$$

Hence the final derivative is

$$
\boxed{
y'(x) 
= \dfrac{4\,e^{2x}}{\bigl(1 + e^{2x}\bigr)^2}\,
\sin\!\Bigl(\dfrac{1 - e^{2x}}{1 + e^{2x}}\Bigr).
}
$$

}\SetValue{Rubric}{%Markdown



}\SetValue{Hint}{%
Solution Goes Here
}\SetValue{Answer}{%

}
\ProcessDATA



