\SetValue{Module}{1}\SetValue{SectionAB}{A}\SetValue{MainChapter}{}\SetValue{SubChapter}{}\SetValue{Contents}{%%
    
Find the derivative of the function.

$y=\sqrt{1+x e^{-2 x}}$

}\SetValue{Concept}{%



}\SetValue{AltText}{%



}\SetValue{Solution}{%

To find the derivative of 

$$
y = \sqrt{1 + x e^{-2x}},
$$

we can write $y$ as 

$$
y = (1 + x e^{-2x})^{\dfrac{1}{2}}.
$$

Using the chain rule, the derivative is

$$
y'(x) 
= \dfrac{1}{2}(1 + x e^{-2x})^{-\dfrac{1}{2}} 
\cdot \dfrac{d}{dx}[1 + x e^{-2x}].
$$

Next, we compute the derivative of the inside term:

$$
\dfrac{d}{dx}[1 + x e^{-2x}]
= e^{-2x} + x \cdot \dfrac{d}{dx}[e^{-2x}]
= e^{-2x} + x(-2 e^{-2x})
= e^{-2x} - 2x e^{-2x}
= e^{-2x}(1 - 2x).
$$

Putting this all together:

$$
y'(x)
= \dfrac{1}{2\sqrt{1 + x e^{-2x}}} \cdot e^{-2x}(1 - 2x)
= \dfrac{e^{-2x}(1 - 2x)}{2 \sqrt{1 + x e^{-2x}}}.
$$

Hence, the derivative is

$$
\boxed{
y'(x) = \dfrac{e^{-2x}\bigl(1 - 2x\bigr)}{2\, \sqrt{1 + x e^{-2x}}}.
}
$$

}\SetValue{Rubric}{%Markdown



}\SetValue{Hint}{%
Solution Goes Here
}\SetValue{Answer}{%

}
\ProcessDATA



