\SetValue{Module}{1}\SetValue{SectionAB}{A}\SetValue{MainChapter}{}\SetValue{SubChapter}{}\SetValue{Contents}{%%
    
Find the derivative of the function.

$f(t)=\tan \left(e^t\right)+e^{\tan t}$

}\SetValue{Concept}{%



}\SetValue{AltText}{%



}\SetValue{Solution}{%

We have 

$$
f(t)=\tan\bigl(e^t\bigr)+e^{\tan t}.
$$

To find its derivative, we apply the sum rule and the chain rule to each term separately.

\textbf{1) Derivative of $\tan(e^t)$}

Let $u = e^t$. Then,
$$
\dfrac{d}{dt}[\tan(u)] = \sec^2(u)\,\dfrac{du}{dt}.
$$
We know $\dfrac{d}{dt}[e^t] = e^t$. Hence,
$$
\dfrac{d}{dt}[\tan(e^t)] 
= \sec^2\bigl(e^t\bigr)\,\cdot e^t.
$$

\textbf{2) Derivative of $e^{\tan t}$}

Let $v = \tan t$. Then,
$$
\dfrac{d}{dt}\bigl[e^v\bigr] 
= e^v \,\dfrac{dv}{dt}.
$$
We know $\dfrac{d}{dt}[\tan t] = \sec^2 t$. Hence,
$$
\dfrac{d}{dt}[e^{\tan t}]
= e^{\tan t}\,\cdot \sec^2 t.
$$

\textbf{Combine both results}

$$
f'(t)
= \dfrac{d}{dt}\bigl[\tan(e^t)\bigr]
+ \dfrac{d}{dt}\bigl[e^{\tan t}\bigr]
= e^t \,\sec^2\bigl(e^t\bigr)
+ e^{\tan t}\,\sec^2 t.
$$

So the derivative is:

$$
\boxed{f'(t) \;=\; e^t \,\sec^2\bigl(e^t\bigr) + e^{\tan t}\,\sec^2 t.}
$$

}\SetValue{Rubric}{%Markdown



}\SetValue{Hint}{%
Solution Goes Here
}\SetValue{Answer}{%

}
\ProcessDATA



