\SetValue{Module}{1}\SetValue{SectionAB}{A}\SetValue{MainChapter}{}\SetValue{SubChapter}{}\SetValue{Contents}{%%
    
Find $y^{\prime}$ and $y^{\prime \prime}$.

$y=\cos \left(x^2\right)$

}\SetValue{Concept}{%



}\SetValue{AltText}{%



}\SetValue{Solution}{%

We have the function

$$
y = \cos\bigl(x^2\bigr).
$$

First derivative $y'$

1. Let $u = x^2$. 

2. Then $y = \cos(u)$.  

3. By the chain rule,  

   $$
   y' = -\sin(u)\,\dfrac{du}{dx} = -\sin(x^2)\cdot 2x = -2x\,\sin(x^2).
   $$

Hence,

$$
\boxed{y' = -2x\,\sin(x^2).}
$$

Second derivative $y''$

We differentiate $y' = -2x\,\sin(x^2)$ with respect to $x$. 

We will need the product rule:

$$
\dfrac{d}{dx}\bigl[f(x)\,g(x)\bigr] 
= f'(x)\,g(x) + f(x)\,g'(x).
$$

- Let $f(x) = -2x$, so $f'(x) = -2.$  

- Let $g(x) = \sin\bigl(x^2\bigr)$. To find $g'(x)$, apply the chain rule again:

  $$
  g'(x) = \cos(x^2)\,\dfrac{d}{dx}\bigl(x^2\bigr) = \cos(x^2)\,(2x) = 2x\,\cos(x^2).
  $$

Thus,

$$
y'' 
= \underbrace{(-2)}_{f'(x)} \,\sin(x^2)
 + \underbrace{(-2x)}_{f(x)} \,\bigl[\,2x\,\cos(x^2)\bigr].
$$

Simplify:

$$
y'' 
= -2\,\sin(x^2) \;-\; 4x^2\,\cos(x^2).
$$

Hence,

$$
\boxed{y'' = -2\,\sin(x^2) \;-\; 4x^2\,\cos(x^2).}
$$

}\SetValue{Rubric}{%Markdown



}\SetValue{Hint}{%
Solution Goes Here
}\SetValue{Answer}{%

}
\ProcessDATA



