\SetValue{Module}{1}\SetValue{SectionAB}{A}\SetValue{MainChapter}{}\SetValue{SubChapter}{}\SetValue{Contents}{%%
    
Find $y^{\prime}$ and $y^{\prime \prime}$.

$y=\cos ^2 x$

}\SetValue{Concept}{%



}\SetValue{AltText}{%



}\SetValue{Solution}{%

We have 

$$
y = \cos^2 x.
$$

A straightforward way to see this is to write $y = \bigl(\cos x\bigr)^2$.

First derivative $y'$

Use the chain rule (or simply treat it as a power rule applied to $\cos x$):

$$
y' = 2\,\cos x \cdot \dfrac{d}{dx}[\cos x] = 2 \cos x \cdot (-\sin x) = -2 \,\sin x \,\cos x.
$$

Often, this is also written in a trigonometric identity form:

$$
-2 \sin x \cos x = -\sin(2x).
$$

So either form is acceptable:

$$
\boxed{y' = -2\,\sin x\,\cos x = -\sin(2x).}
$$

Second derivative $y''$

If we use $y' = -2\,\sin x \cos x$, apply the product rule:

$$
y' = -2\, [\,\sin x \,\cos x\,].
$$

Let $f(x) = \sin x$ and $g(x) = \cos x$. 

Then

$$
\dfrac{d}{dx}[\sin x \,\cos x] = \sin x \cdot (-\sin x) + \cos x \cdot \cos x 
= -\sin^2 x + \cos^2 x 
= \cos(2x).
$$

Hence,

$$
y'' 
= -2 \,\dfrac{d}{dx}[\sin x\,\cos x]
= -2 \,\cos(2x).
$$

Alternatively, starting with $y' = -\sin(2x)$, we immediately get

$$
y'' = -\dfrac{d}{dx}[\sin(2x)] = -\bigl[2\,\cos(2x)\bigr] = -2 \cos(2x).
$$

So,

$$
\boxed{y'' = -2\,\cos(2x).}
$$

}\SetValue{Rubric}{%Markdown



}\SetValue{Hint}{%
Solution Goes Here
}\SetValue{Answer}{%

}
\ProcessDATA



