\SetValue{Module}{1}\SetValue{SectionAB}{A}\SetValue{MainChapter}{}\SetValue{SubChapter}{}\SetValue{Contents}{%%
    
Find $y^{\prime}$ and $y^{\prime \prime}$.

$y=e^{e^x}$

}\SetValue{Concept}{%



}\SetValue{AltText}{%



}\SetValue{Solution}{%

We are given:

$$
y = e^{e^x}
$$

We are to find the first and second derivatives: $ y'$ and $ y''$.

\textbf{Step 1: First Derivative $ y'$}

Use the **chain rule**:

Letâ€™s define:

- Let $ u = e^x$, so $ y = e^u$

- Then $ \dfrac{dy}{dx} = \dfrac{dy}{du} \cdot \dfrac{du}{dx}$

So:

$$
y' = \dfrac{d}{dx}(e^{e^x}) = e^{e^x} \cdot \dfrac{d}{dx}(e^x) = e^{e^x} \cdot e^x
$$

\textbf{Step 2: Second Derivative $ y''$}

Now differentiate $ y' = e^{e^x} \cdot e^x$ using the **product rule**:

Let:

- $ f(x) = e^{e^x}$

- $ g(x) = e^x$

Then:

$$
y'' = f'(x) \cdot g(x) + f(x) \cdot g'(x)
$$

We already know:

- $ f(x) = e^{e^x} \Rightarrow f'(x) = e^{e^x} \cdot e^x$

- $ g(x) = e^x \Rightarrow g'(x) = e^x$

Now plug in:

$$
y'' = (e^{e^x} \cdot e^x) \cdot e^x + e^{e^x} \cdot e^x
= e^{e^x} \cdot e^{2x} + e^{e^x} \cdot e^x
= e^{e^x} \left( e^{2x} + e^x \right)
$$

\textbf{Final Answers:}

$$
\boxed{
\begin{aligned}
y' &= e^{e^x} \cdot e^x \\
y'' &= e^{e^x} \left( e^{2x} + e^x \right)
\end{aligned}
}
$$

}\SetValue{Rubric}{%Markdown



}\SetValue{Hint}{%
Solution Goes Here
}\SetValue{Answer}{%

}
\ProcessDATA



