\SetValue{Module}{1}\SetValue{SectionAB}{A}\SetValue{MainChapter}{}\SetValue{SubChapter}{}\SetValue{Contents}{%%

Find an equation of the tangent line to the curve $y=\dfrac{2}{\left(1+e^{-x}\right)}$ at the point $(0,1)$.

}\SetValue{Concept}{%



}\SetValue{AltText}{%



}\SetValue{Solution}{%

We are given:

- Function: $ y = \dfrac{2}{1 + e^{-x}}$

- Point: $ (0, 1)$

We want the equation of the tangent line at that point.

Step 1: Differentiate $ y$

We’ll use the quotient rule (or chain rule via rewriting):

Option: Rewrite first

Let’s write:

$$
y = 2(1 + e^{-x})^{-1}
$$

Differentiate using the chain rule:

$$
y' = 2 \cdot (-1)(1 + e^{-x})^{-2} \cdot \dfrac{d}{dx}(1 + e^{-x})
= -2(1 + e^{-x})^{-2} \cdot (-e^{-x})
$$

$$
y' = \dfrac{2e^{-x}}{(1 + e^{-x})^2}
$$

Step 2: Evaluate derivative at $ x = 0$

$$
y'(0) = \dfrac{2e^{0}}{(1 + e^{0})^2} = \dfrac{2 \cdot 1}{(1 + 1)^2} = \dfrac{2}{4} = \dfrac{1}{2}
$$

So the slope of the tangent line is $ \dfrac{1}{2}$.

Step 3: Use point-slope form

Point: $ (0, 1)$, Slope: $ \dfrac{1}{2}$

$$
y - 1 = \dfrac{1}{2}(x - 0) \Rightarrow y = \dfrac{1}{2}x + 1
$$

Final Answer:

$$
\boxed{y = \dfrac{1}{2}x + 1}
$$

}\SetValue{Rubric}{%Markdown



}\SetValue{Hint}{%
Solution Goes Here
}\SetValue{Answer}{%

}
\ProcessDATA



