\SetValue{Module}{1}\SetValue{SectionAB}{A}\SetValue{MainChapter}{}\SetValue{SubChapter}{}\SetValue{Contents}{%%
    
Follow the steps below to solve

$$
y^{\prime}=-3 y+5, \quad y(0)=1
$$

(c) Use the potential function to find the general solution of the differential equation.

}\SetValue{Concept}{%



}\SetValue{AltText}{%



}\SetValue{Solution}{%

We have transformed the differential equation $y^{\prime}=-3 y+5$ into the form $\psi^{\prime}=0$, where $\psi(t, y)=$ $e^{3 t} y-\frac{5}{3} e^{3 t}$, from part (b).

Now, to find the general solution of the differential equation, we integrate the equation $\psi^{\prime}(t)=0$ with respect to $t$:

$$
\begin{gathered}
\int \psi^{\prime}(t) d t=\int 0 d t \\
\psi(t)=C
\end{gathered}
$$

where $C$ is the constant of integration.

Substitute the expression for $\psi(t, y)$ back into this integrated equation:

$$
e^{3 t} y-\frac{5}{3} e^{3 t}=C
$$


Now, solve this equation for $y(t)$ to find the general solution:

$\$ e^{3 t} y=C+\frac{5}{3} e^{3 t} \$$ Divide both sides by $e^{3 t}$:

$$
\begin{aligned}
& y(t)=\frac{C+\frac{5}{3} e^{3 t}}{e^{3 t}} \\
& y(t)=\frac{C}{e^{3 t}}+\frac{\frac{5}{3} e^{3 t}}{e^{3 t}} \\
& y(t)=C e^{-3 t}+\frac{5}{3}
\end{aligned}
$$


This is the general solution to the differential equation $y^{\prime}=-3 y+5$.

The final answer is $y(t)=C e^{-3 t}+\frac{5}{3}, \quad$ for all $C \in \mathbb{R}$.

}\SetValue{Rubric}{%Markdown



}\SetValue{Hint}{%
Solution Goes Here
}\SetValue{Answer}{%

}
\ProcessDATA



