\SetValue{Module}{1}\SetValue{SectionAB}{A}\SetValue{MainChapter}{}\SetValue{SubChapter}{}\SetValue{Contents}{%%
    
Follow the steps below to solve

$$
y^{\prime}=-3 y+5, \quad y(0)=1
$$

(d) Find the solution of the initial value problem above.

}\SetValue{Concept}{%



}\SetValue{AltText}{%



}\SetValue{Solution}{%

From part (c), the general solution of the differential equation $y^{\prime}=-3 y+5$ is:

$$
y(t)=C e^{-3 t}+\frac{5}{3}
$$

where $C$ is the constant of integration.

Now, we use the initial condition $y(0)=1$ to find the specific value of $C$ for this initial value problem.

Substitute $t=0$ and $y=1$ into the general solution:

$$
1=C e^{-3(0)}+\frac{5}{3}
$$

$\$ 1=C e^0+\frac{5}{3} \$$ Since $e^0=1:$

$$
\begin{gathered}
1=C(1)+\frac{5}{3} \\
1=C+\frac{5}{3}
\end{gathered}
$$


Now, solve for $C$:

$$
C=1-\frac{5}{3}=\frac{3}{3}-\frac{5}{3}=-\frac{2}{3}
$$


Substitute the value of $C=-\frac{2}{3}$ back into the general solution:

$$
y(t)=-\frac{2}{3} e^{-3 t}+\frac{5}{3}
$$


This is the solution to the initial value problem $y^{\prime}=-3 y+5, \quad y(0)=1$.

The final answer is $y(t)=-\frac{2}{3} e^{-3 t}+\frac{5}{3}$.

}\SetValue{Rubric}{%Markdown



}\SetValue{Hint}{%
Solution Goes Here
}\SetValue{Answer}{%

}
\ProcessDATA



