\SetValue{Module}{1}\SetValue{SectionAB}{A}\SetValue{MainChapter}{}\SetValue{SubChapter}{}\SetValue{Contents}{%%
    
Find constants $a, b$, so that

$$
y(t)=(t+3) e^{2 t}
$$

is solution of the IVP

$$
y^{\prime}=a y+e^{2 t}, \quad y(0)=b.
$$

}\SetValue{Concept}{%



}\SetValue{AltText}{%



}\SetValue{Solution}{%

We are given the function:

$$
y(t)=(t+3) e^{2 t}
$$

and the initial value problem (IVP):

$$
y^{\prime}=a y+e^{2 t}, \quad y(0)=b
$$


We are to find constants $a$ and $b$ so that $y(t)$ solves this IVP.

Step 1: Compute $y^{\prime}(t)$

Use the product rule:

$$
\begin{gathered}
y(t)=(t+3) e^{2 t} \quad \Rightarrow \quad y^{\prime}(t)=\frac{d}{d t}\left[(t+3) e^{2 t}\right] \\
y^{\prime}(t)=(t+3) \cdot \frac{d}{d t}\left[e^{2 t}\right]+e^{2 t} \cdot \frac{d}{d t}[t+3]=(t+3)\left(2 e^{2 t}\right)+e^{2 t}(1)=2(t+3) e^{2 t}+e^{2 t} \\
\Rightarrow y^{\prime}(t)=[2(t+3)+1] e^{2 t}=(2 t+7) e^{2 t}
\end{gathered}
$$

Step 2: Express $y^{\prime}$ as $a y+e^{2 t}$

We are told:

$$
y^{\prime}=a y+e^{2 t}
$$


From earlier:

- $y(t)=(t+3) e^{2 t}$

- $y^{\prime}(t)=(2 t+7) e^{2 t}$

Plug into the differential equation:

$$
(2 t+7) e^{2 t}=a \cdot(t+3) e^{2 t}+e^{2 t}
$$


Divide both sides by $e^{2 t}$ (since $e^{2 t} \neq 0$ ):

$$
2 t+7=a(t+3)+1
$$


Simplify right-hand side:

$$
a(t+3)+1=a t+3 a+1
$$


Match both sides:

$$
2 t+7=a t+3 a+1
$$


Equating coefficients:

- Coefficient of $t: a=2$

- Constant term: $3 a+1=7 \Rightarrow 3 a=6 \Rightarrow a=2$ (confirmed)

Step 3: Compute $b=y(0)$

From $y(t)=(t+3) e^{2 t}$, plug in $t=0$:

$$
y(0)=(0+3) e^0=3 \cdot 1=3 \Rightarrow b=3
$$


Final Answer:

$$
a=2, \quad b=3
$$


}\SetValue{Rubric}{%Markdown



}\SetValue{Hint}{%
Solution Goes Here
}\SetValue{Answer}{%

}
\ProcessDATA



