\SetValue{Module}{1}\SetValue{SectionAB}{A}\SetValue{MainChapter}{}\SetValue{SubChapter}{}\SetValue{Contents}{%%
    
Find the solution of the IVP

$$
y^{\prime}=-4 y+2, \quad y(0)=5
$$

}\SetValue{Concept}{%



}\SetValue{AltText}{%



}\SetValue{Solution}{%

Let's solve the initial value problem $y^{\prime}=-4 y+2$, with $y(0)=5$ using the integrating factor method.

First, rewrite the differential equation in the standard linear first-order form:

$\$ y^{\prime}+P(t) y=Q(t) \$$ The given equation is $y^{\prime}=-4 y+2$. Move the term involving $y$ to the left side:

$$
y^{\prime}+4 y=2
$$


Here, we can identify $P(t)=4$ and $Q(t)=2$.

Next, calculate the integrating factor, $I(t)$, using the formula $I(t)=e^{\int P(t) d t}$:

$$
I(t)=e^{\int 4 d t}=e^{4 t}
$$


Now, multiply the standard form of the differential equation by the integrating factor:

$$
e^{4 t}\left(y^{\prime}+4 y\right)=e^{4 t}(2)
$$

$\$ e^{4 t} y^{\prime}+4 e^{4 t} y=2 e^{4 t} \$$ The left side of this equation is the derivative of the product of the integrating factor and $y(t)$, i.e., $\frac{d}{d t}\left(e^{4 t} y\right)$. So, we can write:

$$
\frac{d}{d t}\left(e^{4 t} y\right)=2 e^{4 t}
$$


Now, integrate both sides with respect to $t$:

$$
\begin{gathered}
\int \frac{d}{d t}\left(e^{4 t} y\right) d t=\int 2 e^{4 t} d t \\
e^{4 t} y=2 \int e^{4 t} d t \\
e^{4 t} y=2\left(\frac{1}{4} e^{4 t}\right)+C
\end{gathered}
$$


$$
e^{4 t} y=\frac{1}{2} e^{4 t}+C
$$

where $C$ is the constant of integration.

Now, solve for $y(t)$ by dividing both sides by $e^{4 t}$:

$$
\begin{aligned}
& y(t)=\frac{\frac{1}{2} e^{4 t}+C}{e^{4 t}} \\
& y(t)=\frac{1}{2}+C e^{-4 t}
\end{aligned}
$$


This is the general solution to the differential equation.

Finally, use the initial condition $y(0)=5$ to find the value of $C$. Substitute $t=0$ and $y=5$ into the general solution:

$$
\begin{gathered}
5=\frac{1}{2}+C e^{-4(0)} \\
5=\frac{1}{2}+C e^0 \\
5=\frac{1}{2}+C(1) \\
5=\frac{1}{2}+C \\
C=5-\frac{1}{2}=\frac{10}{2}-\frac{1}{2}=\frac{9}{2}
\end{gathered}
$$


Substitute the value of $C=\frac{9}{2}$ back into the general solution to get the particular solution for the IVP:

$$
y(t)=\frac{1}{2}+\frac{9}{2} e^{-4 t}
$$


Rearranging the terms, we get:

$$
y(t)=\frac{9}{2} e^{-4 t}+\frac{1}{2}
$$


The final answer is $y(t)=\frac{9}{2} e^{-4 t}+\frac{1}{2}$.





}\SetValue{Rubric}{%Markdown



}\SetValue{Hint}{%
Solution Goes Here
}\SetValue{Answer}{%

}
\ProcessDATA



