\SetValue{Module}{1}\SetValue{SectionAB}{A}\SetValue{MainChapter}{}\SetValue{SubChapter}{}\SetValue{Contents}{%%
    
Find the solution of the IVP

$$
\frac{d y}{d t}(t)=3 y(t)-2, \quad y(1)=1
$$

}\SetValue{Concept}{%



}\SetValue{AltText}{%



}\SetValue{Solution}{%

The given initial value problem (IVP) is:

$$
\frac{d y}{d t}(t)=3 y(t)-2, \quad y(1)=1
$$


This is a first-order linear ordinary differential equation.
We can solve it by separating variables or by using an integrating factor. We previously solved this using separation of variables.

The differential equation is $\frac{d y}{d t}=3 y-2$.

Separating variables, we get $\frac{d y}{3 y-2}=d t$.
Integrating both sides:

$$
\begin{gathered}
\int \frac{d y}{3 y-2}=\int d t \\
\frac{1}{3} \ln |3 y-2|=t+C_1 \\
\ln |3 y-2|=3 t+3 C_1 \\
|3 y-2|=e^{3 t+3 C_1}=e^{3 C_1} e^{3 t}
\end{gathered}
$$

$\$ 3 y-2=C e^{3 t} \$$ where $C= \pm e^{3 C_1}$ or $C=0$.

$$
3 y=C e^{3 t}+2
$$

$ y(t)=\frac{C}{3} e^{3 t}+\frac{2}{3}$ Let $A=\frac{C}{3}$. 

The general solution is:

$$
y(t)=A e^{3 t}+\frac{2}{3}
$$


Now, we use the initial condition $y(1)=1$ to find the value of $A$. Substitute $t=1$ and $y=1$ into the general solution:

$$
\begin{gathered}
1=A e^{3(1)}+\frac{2}{3} \\
1=A e^3+\frac{2}{3} \\
1-\frac{2}{3}=A e^3 \\
\frac{1}{3}=A e^3 \\
A=\frac{1}{3 e^3}=\frac{1}{3} e^{-3}
\end{gathered}
$$

Substitute the value of $A$ back into the general solution:

$$
\begin{aligned}
& y(t)=\frac{1}{3} e^{-3} e^{3 t}+\frac{2}{3} \\
& y(t)=\frac{1}{3} e^{3 t-3}+\frac{2}{3} \\
& y(t)=\frac{1}{3} e^{3(t-1)}+\frac{2}{3}
\end{aligned}
$$


The solution of the initial value problem is $y(t)=\frac{1}{3} e^{3(t-1)}+\frac{2}{3}$.

The final answer is $y(t)=\frac{1}{3} e^{3(t-1)}+\frac{2}{3}$.

}\SetValue{Rubric}{%Markdown



}\SetValue{Hint}{%
Solution Goes Here
}\SetValue{Answer}{%

}
\ProcessDATA



