\SetValue{Module}{1}\SetValue{SectionAB}{A}\SetValue{MainChapter}{}\SetValue{SubChapter}{}\SetValue{Contents}{%%
  
Find all solutions of the equation

$$
y^{\prime}=-x y+6 x \sqrt{y}
$$

}\SetValue{Concept}{%



}\SetValue{AltText}{%



}\SetValue{Solution}{%

Step 1: Recognize Bernoulli Form

We rewrite the equation as:

$$
y^{\prime}+x y=6 x y^{1 / 2}
$$


This is a Bernoulli equation of the form:

$$
y^{\prime}+a(x) y=b(x) y^n
$$

with:

- $a(x)=x$

- $b(x)=6 x$

- $n=\frac{1}{2}$

Step 2: Bernoulli Substitution

Let:

$$
v=y^{1-n}=y^{1 / 2}=\sqrt{y} \quad \Rightarrow \quad y=v^2, \quad y^{\prime}=2 v v^{\prime}
$$


Substitute into the equation:

$$
2 v v^{\prime}+x v^2=6 x v \Rightarrow v v^{\prime}+\frac{x}{2} v^2=3 x v
$$


Divide by $v \neq 0$ :

$$
v^{\prime}+\frac{x}{2} v=3 x
$$

Step 3: Solve the Linear Equation

This is a linear ODE:

$$
v^{\prime}+\frac{x}{2} v=3 x
$$


Integrating factor:

$$
\mu(x)=e^{\int \frac{x}{2} d x}=e^{x^2 / 4}
$$


Multiply both sides:

$$
\frac{d}{d x}\left(e^{x^2 / 4} v\right)=3 x e^{x^2 / 4}
$$


Integrate:

$$
e^{x^2 / 4} v=\int 3 x e^{x^2 / 4} d x=6 e^{x^2 / 4}+C \Rightarrow v=6+C e^{-x^2 / 4}
$$


Step 4: Back-substitute

Since $v=\sqrt{y}$, we have:

$$
y=v^2=\left(6+C e^{-x^2 / 4}\right)^2
$$


}\SetValue{Rubric}{%Markdown



}\SetValue{Hint}{%
Solution Goes Here
}\SetValue{Answer}{%

}
\ProcessDATA



