\SetValue{Module}{1}\SetValue{SectionAB}{A}\SetValue{MainChapter}{}\SetValue{SubChapter}{}\SetValue{Contents}{%%
  
Find all solutions of

$$
y^{\prime}=a y+b y^n,
$$

where $a \neq 0, b$, and $n$ are real constants with $n \neq 0,1$.

}\SetValue{Concept}{%



}\SetValue{AltText}{%



}\SetValue{Solution}{%

We are asked to solve the general nonlinear differential equation:

$$
y^{\prime}=a y+b y^n
$$

where $a \neq 0, b \in \mathbb{R}$, and $n \neq 0,1$. This is a Bernoulli differential equation, which can be solved by a standard substitution.

Step 1: Recognize Bernoulli Form
This is of the form:

$$
y^{\prime}=a y+b y^n
$$


We can write it as:

$$
y^{\prime}-a y=b y^n
$$


This matches the standard Bernoulli equation:

$$
y^{\prime}+P(x) y=Q(x) y^n
$$


Step 2: Use Bernoulli Substitution

Let:

$$
v=y^{1-n} \quad \Rightarrow \quad y=v^{\frac{1}{1-n}}
$$


Differentiate both sides using the chain rule:

$$
y^{\prime}=\frac{1}{1-n} v^{\frac{n}{1-n}} v^{\prime}
$$

Now recall from the original equation:

$$
y^{\prime}-a y=b y^n
$$


Substitute $y=v^{1 /(1-n)}$, and notice that:
- $y=v^{1 /(1-n)}$
- $y^n=v^{n /(1-n)}$

So:

$$
\frac{1}{1-n} v^{\frac{n}{1-n}} v^{\prime}-a v^{\frac{1}{1-n}}=b v^{\frac{n}{1-n}}
$$


Multiply both sides by $(1-n) v^{-\frac{n}{1-n}}$ :

$$
v^{\prime}-a(1-n) v=b(1-n)
$$


This is now a first-order linear equation in $v$ :

$$
v^{\prime}-a(1-n) v=b(1-n)
$$


Step 3: Solve the Linear Equation

Let's solve:

$$
v^{\prime}-A v=B, \quad \text { where } A=a(1-n), \quad B=b(1-n)
$$


This is a standard linear ODE. The integrating factor is:

$$
\mu(x)=e^{-A x}=e^{-a(1-n) x}
$$


Multiply through:

$$
\frac{d}{d x}\left(e^{-A x} v\right)=B e^{-A x}
$$


Integrate both sides:

$$
e^{-A x} v=\int B e^{-A x} d x=-\frac{B}{A} e^{-A x}+C \Rightarrow v(x)=-\frac{B}{A}+C e^{A x}
$$


Now plug back in:

$$
v(x)=-\frac{b(1-n)}{a(1-n)}+C e^{a(1-n) x}=-\frac{b}{a}+C e^{a(1-n) x}
$$


Step 4: Back-substitute $v=y^{1-n}$

$$
y^{1-n}=-\frac{b}{a}+C e^{a(1-n) x} \Rightarrow y(x)=\left(-\frac{b}{a}+C e^{a(1-n) x}\right)^{\frac{1}{1-n}}
$$

Final Answer:

$$
y(x)=\left(-\frac{b}{a}+C e^{a(1-n) x}\right)^{\frac{1}{1-n}}, \quad C \in \mathbb{R}
$$


This is the general solution of the equation

$$
y^{\prime}=a y+b y^n
$$

for $n \neq 0,1$ and $a \neq 0$

}\SetValue{Rubric}{%Markdown



}\SetValue{Hint}{%
Solution Goes Here
}\SetValue{Answer}{%

}
\ProcessDATA



