\SetValue{Module}{1}\SetValue{SectionAB}{A}\SetValue{MainChapter}{}\SetValue{SubChapter}{}\SetValue{Contents}{%%
    
Find the general solution of

$$
y^{\prime}=-y+e^{-2 t}
$$

}\SetValue{Concept}{%



}\SetValue{AltText}{%



}\SetValue{Solution}{%

using Theorem 1.2.1 (Variable Coefficients) from section 1.2.2, which provides a formula for solving first-order linear differential equations of the form

$$
y^{\prime}=a(t) y+b(t)
$$


Step 1: Match to the standard form

We rewrite the equation as:

$$
y^{\prime}=(-1) \cdot y+e^{-2 t}
$$


Thus:

- $a(t)=-1$

- $b(t)=e^{-2 t}$

Step 2: Apply the theorem

We are told that the general solution is:

$$
y(t)=c e^{A(t)}+e^{A(t)} \int e^{-A(t)} b(t) d t
$$

where:

$$
A(t)=\int a(t) d t=\int-1 d t=-t
$$


Step 3: Plug into the formula

$$
y(t)=c e^{-t}+e^{-t} \int e^t \cdot e^{-2 t} d t
$$


Simplify the integrand:

$$
e^t \cdot e^{-2 t}=e^{-t}
$$


So the integral becomes:

$$
\int e^{-t} d t=-e^{-t}+C_1
$$


But we only need one constant of integration (the $c$ already covers it), so we drop $C_1$.

Then:

$$
y(t)=c e^{-t}+e^{-t}\left(-e^{-t}\right)=c e^{-t}-e^{-2 t}
$$


Final Answer:

$$
y(t)=c e^{-t}-e^{-2 t}, \quad c \in \mathbb{R}
$$



}\SetValue{Rubric}{%Markdown



}\SetValue{Hint}{%
Solution Goes Here
}\SetValue{Answer}{%

}
\ProcessDATA



