\SetValue{Module}{1}\SetValue{SectionAB}{A}\SetValue{MainChapter}{}\SetValue{SubChapter}{}\SetValue{Contents}{%%
  
Find the solution $y$ to the IVP

$$
y^{\prime}=y+2 t e^{2 t}, \quad y(0)=0
$$

}\SetValue{Concept}{%



}\SetValue{AltText}{%



}\SetValue{Solution}{%

using Theorem 1.2.3 (Variable Coefficients IVP) from section 1.2.3, which gives an explicit formula for the unique solution of the initial value problem:

Step 1: Identify the components of the IVP
We are given:
- Differential equation: $y^{\prime}=a(t) y+b(t)$
- Initial condition: $\quad y(0)=0$

From the equation:
- $a(t)=1$
- $b(t)=2 t e^{2 t}$
- $t_0=0$
- $y_0=0$

Step 2: Compute $A(t)=\int_{t_0}^t a(s) d s$

$$
A(t)=\int_0^t 1 d s=t
$$


Step 3: Use the theorem's formula
The unique solution is:

$$
y(t)=y_0 e^{A(t)}+e^{A(t)} \int_{t_0}^t e^{-A(s)} b(s) d s
$$


Substitute the known values:

$$
y(t)=0 \cdot e^t+e^t \int_0^t e^{-s} \cdot 2 s e^{2 s} d s
$$


Simplify the integrand:

$$
e^{-s} \cdot 2 s e^{2 s}=2 s e^s
$$

So:

$$
y(t)=e^t \int_0^t 2 s e^s d s
$$


Step 4: Evaluate the integral $\int_0^t 2 s e^s d s$
Use integration by parts:
Let:
- $u=2 s \Rightarrow d u=2 d s$
- $d v=e^s d s \Rightarrow v=e^s$

Then:

$$
\int 2 s e^s d s=2 s e^s-\int 2 e^s d s=2 s e^s-2 e^s+C
$$


Thus:

$$
\int_0^t 2 s e^s d s=\left[2 s e^s-2 e^s\right]_0^t=\left(2 t e^t-2 e^t\right)-\left(0-2 e^0\right)=2 t e^t-2 e^t+2
$$


Step 5: Final expression for $y(t)$

$$
y(t)=e^t \cdot\left(2 t e^t-2 e^t+2\right)=2 t e^{2 t}-2 e^{2 t}+2 e^t
$$


Final Answer:

$$
y(t)=2 e^t+2(t-1) e^{2 t}
$$



}\SetValue{Rubric}{%Markdown



}\SetValue{Hint}{%
Solution Goes Here
}\SetValue{Answer}{%

}
\ProcessDATA



