\SetValue{Module}{1}\SetValue{SectionAB}{A}\SetValue{MainChapter}{}\SetValue{SubChapter}{}\SetValue{Contents}{%%
  
Find the solution $y$ to the IVP

$$
t y^{\prime}+2 y=\frac{\sin (t)}{t}, \quad y\left(\frac{\pi}{2}\right)=\frac{2}{\pi}
$$

for $t>0$.

}\SetValue{Concept}{%



}\SetValue{AltText}{%



}\SetValue{Solution}{%

Step 1: Write in standard linear form
Divide both sides by $t$ (since $t>0$ ):

$$
y^{\prime}+\frac{2}{t} y=\frac{\sin t}{t^2}
$$


This is a first-order linear equation with variable coefficients, of the form:

$$
y^{\prime}+a(t) y=b(t)
$$

where:
- $a(t)=\frac{2}{t}$
- $b(t)=\frac{\sin t}{t^2}$

Step 2: Compute the integrating factor

$$
\mu(t)=e^{\int a(t) d t}=e^{\int \frac{2}{t} d t}=e^{2 \ln t}=t^2
$$


Step 3: Multiply through by the integrating factor

$$
t^2 y^{\prime}+2 t y=\sin t
$$


Left-hand side is the derivative of $t^2 y$ :

$$
\frac{d}{d t}\left(t^2 y\right)=\sin t
$$


Step 4: Integrate both sides

$$
\begin{gathered}
\int \frac{d}{d t}\left(t^2 y\right) d t=\int \sin t d t \\
t^2 y=-\cos t+C
\end{gathered}
$$

Step 5: Solve for $y(t)$

$$
y(t)=\frac{-\cos t+C}{t^2}
$$


Step 6: Apply initial condition
We are given:

$$
y\left(\frac{\pi}{2}\right)=\frac{2}{\pi}
$$


Substitute:

$$
\begin{aligned}
& \frac{2}{\pi}=\frac{-\cos \left(\frac{\pi}{2}\right)+C}{\left(\frac{\pi}{2}\right)^2} \\
& \frac{2}{\pi}=\frac{0+C}{\left(\frac{\pi^2}{4}\right)}=\frac{4 C}{\pi^2}
\end{aligned}
$$


Solve for $C$ :

$$
\frac{2}{\pi}=\frac{4 C}{\pi^2} \quad \Rightarrow \quad C=\frac{2}{\pi} \cdot \frac{\pi^2}{4}=\frac{\pi}{2}
$$


Final Answer:

$$
y(t)=\frac{-\cos t+\frac{\pi}{2}}{t^2}

=\frac{\pi}{2 t^2}-\frac{\cos (t)}{t^2}
$$


This is the unique solution to the IVP for $t>0$.


}\SetValue{Rubric}{%Markdown



}\SetValue{Hint}{%
Solution Goes Here
}\SetValue{Answer}{%

}
\ProcessDATA



