\SetValue{Module}{1}\SetValue{SectionAB}{A}\SetValue{MainChapter}{}\SetValue{SubChapter}{}\SetValue{Contents}{%%
  
Find all solutions $y$ to the ODE

$$
t y^{\prime}+n y=t^2
$$

with $n$ a positive integer.

}\SetValue{Concept}{%



}\SetValue{AltText}{%



}\SetValue{Solution}{%

Step 1: Write in standard linear form
Divide both sides by $t$ (assume $t>0$ or $t<0$, but $t \neq 0$ ):

$$
y^{\prime}+\frac{n}{t} y=t
$$


This is of the form:

$$
y^{\prime}+a(t) y=b(t), \quad \text { with } a(t)=\frac{n}{t}, \quad b(t)=t
$$


Step 2: Compute the integrating factor

$$
\mu(t)=e^{\int \frac{n}{t} d t}=e^{n \ln |t|}=|t|^n
$$

(We'll work with $t>0$ so $\mu(t)=t^n$.)

Step 3: Multiply through by integrating factor

$$
t^n y^{\prime}+n t^{n-1} y=t^{n+1}
$$


Left-hand side is:

$$
\frac{d}{d t}\left(t^n y\right)
$$


So:

$$
\frac{d}{d t}\left(t^n y\right)=t^{n+1}
$$


Step 4: Integrate both sides

$$
\begin{gathered}
\int \frac{d}{d t}\left(t^n y\right) d t=\int t^{n+1} d t \\
t^n y=\frac{t^{n+2}}{n+2}+C
\end{gathered}
$$

Step 5: Solve for $y(t)$

$$
y(t)=\frac{t^{n+2}}{(n+2) t^n}+\frac{C}{t^n}=\frac{t^2}{n+2}+C t^{-n}
$$


Final Answer:

$$
y(t)=\frac{t^2}{n+2}+C t^{-n}=\frac{t^2}{n+2}+\frac{c}{t^n}, \quad t \neq 0, C \in \mathbb{R}
$$



}\SetValue{Rubric}{%Markdown



}\SetValue{Hint}{%
Solution Goes Here
}\SetValue{Answer}{%

}
\ProcessDATA



