\SetValue{Module}{1}\SetValue{SectionAB}{A}\SetValue{MainChapter}{}\SetValue{SubChapter}{}\SetValue{Contents}{%%
  
Find all solutions of the equation

$$
y^{\prime}=y-2 \sin (t)
$$

}\SetValue{Concept}{%



}\SetValue{AltText}{%



}\SetValue{Solution}{%

Step 1: Write in standard form

$$
y^{\prime}-y=-2 \sin (t)
$$


This is of the form:

$$
y^{\prime}+a(t) y=b(t), \quad \text { with } a(t)=-1, \quad b(t)=-2 \sin (t)
$$


Step 2: Find the integrating factor

$$
\mu(t)=e^{\int-1 d t}=e^{-t}
$$


Step 3: Multiply both sides by the integrating factor

$$
e^{-t} y^{\prime}-e^{-t} y=-2 e^{-t} \sin (t)
$$


Left-hand side becomes:

$$
\frac{d}{d t}\left(e^{-t} y\right)=-2 e^{-t} \sin (t)
$$


Step 4: Integrate both sides

$$
\int \frac{d}{d t}\left(e^{-t} y\right) d t=\int-2 e^{-t} \sin (t) d t
$$


We need to compute:

$$
\int-2 e^{-t} \sin (t) d t
$$


This is a standard integral. The formula is:

$$
\int e^{a t} \sin (b t) d t=\frac{e^{a t}}{a^2+b^2}(a \sin (b t)-b \cos (b t))
$$


Using $a=-1, b=1$, we get:

$$
\int e^{-t} \sin (t) d t=\frac{e^{-t}}{2}(-\sin (t)-\cos (t))
$$


So:

$$
\int-2 e^{-t} \sin (t) d t=-2 \cdot \frac{e^{-t}}{2}(-\sin (t)-\cos (t))=e^{-t}(\sin (t)+\cos (t))
$$

Step 5: Solve for $y(t)$

$$
e^{-t} y=e^{-t}(\sin (t)+\cos (t))+C
$$


Multiply both sides by $e^t$ :

$$
y(t)=\sin (t)+\cos (t)+C e^t
$$


Final Answer:

$$
y(t)=\sin (t)+\cos (t)+C e^t, \quad C \in \mathbb{R}
$$



}\SetValue{Rubric}{%Markdown



}\SetValue{Hint}{%
Solution Goes Here
}\SetValue{Answer}{%

}
\ProcessDATA



