\SetValue{Module}{1}\SetValue{SectionAB}{A}\SetValue{MainChapter}{}\SetValue{SubChapter}{}\SetValue{Contents}{%%
  
Find the solution to the initial value problem

$$
t y^{\prime}=2 y+4 t^3 \cos (4 t), \quad y\left(\frac{\pi}{8}\right)=0
$$

}\SetValue{Concept}{%



}\SetValue{AltText}{%



}\SetValue{Solution}{%

Step 1: Standard form
Divide both sides by $t$ (assuming $t \neq 0$ ):

$$
y^{\prime}-\frac{2}{t} y=4 t^2 \cos (4 t)
$$


This is a first-order linear differential equation in standard form:

$$
y^{\prime}+a(t) y=b(t)
$$

with:
- $a(t)=-\frac{2}{t}$
- $b(t)=4 t^2 \cos (4 t)$

Step 2: Find the integrating factor

$$
\mu(t)=e^{\int a(t) d t}=e^{\int-\frac{2}{t} d t}=e^{-2 \ln |t|}=t^{-2}
$$

(We can assume $t>0$ since $\frac{\pi}{8}>0$.)

Step 3: Multiply both sides by the integrating factor

$$
t^{-2} y^{\prime}-\frac{2}{t^3} y=4 \cos (4 t)
$$


Left-hand side is:

$$
\frac{d}{d t}\left(t^{-2} y\right)
$$


So:

$$
\frac{d}{d t}\left(t^{-2} y\right)=4 \cos (4 t)
$$


Step 4: Integrate both sides

$$
\begin{gathered}
\int \frac{d}{d t}\left(t^{-2} y\right) d t=\int 4 \cos (4 t) d t \\
t^{-2} y=\int 4 \cos (4 t) d t=\int 4 \cos (4 t) d t=\frac{4}{4} \sin (4 t)+C=\sin (4 t)+C
\end{gathered}
$$

Step 5: Solve for $y(t)$

$$
y(t)=t^2(\sin (4 t)+C)
$$


Step 6: Apply the initial condition $y\left(\frac{\pi}{8}\right)=0$

$$
0=\left(\frac{\pi}{8}\right)^2(\sin (\pi / 2)+C)=\left(\frac{\pi}{8}\right)^2(1+C)
$$


Since $\left(\frac{\pi}{8}\right)^2 \neq 0$, we must have:

$$
1+C=0 \Rightarrow C=-1
$$


Final Answer:

$$
y(t)=t^2(\sin (4 t)-1)=-t^2+t^2 \sin (4 t)
$$



}\SetValue{Rubric}{%Markdown



}\SetValue{Hint}{%
Solution Goes Here
}\SetValue{Answer}{%

}
\ProcessDATA



